<?xml version="1.0" encoding="UTF-8"?>

<section xml:id="sec-precalc-factor" xmlns:xi="http://www.w3.org/2001/XInclude">
  <title>Factoring</title>

  <p>
    Factoring is one of the most important algebra skills for calculus.
    Many problems in limits, derivatives, and integrals require expressions
    to be simplified before any calculus ideas can be applied.
    In this section, we review the most common factoring techniques,
    starting from very basic patterns and gradually building toward
    the types of expressions that appear in calculus problems.
  </p>

  <!-- ======================================================= -->
  <subsection xml:id="ssec-factor-gcf">
    <title>Factoring Out a Greatest Common Factor</title>

    <p>
      The first and most important factoring technique is factoring out
      the greatest common factor.
      If every term in an expression shares a common factor,
      that factor can be factored out.
    </p>

    <principle xml:id="pr-factor-gcf">
      <statement>
        <p>
          If every term of an expression contains a factor <m>a</m>, then
        </p>
        <me>
\begin{array}{rcl}
ab + ac &amp; = &amp; a(b + c)
\end{array}
        </me>
      </statement>
    </principle>

    <example>
      <statement>
        <p>
          Factor <m>6x + 12</m>.
        </p>
      </statement>
      <solution>
        <p>
          Both terms share a factor of <m>6</m>.
        </p>
        <me>
\begin{array}{rcl}
6x + 12 &amp; = &amp; 6(x + 2)
\end{array}
        </me>
      </solution>
    </example>

    <example>
      <statement>
        <p>
          Factor <m>4x^2 + 8x</m>.
        </p>
      </statement>
      <solution>
        <p>
          Both terms share a factor of <m>4x</m>.
        </p>
        <me>
\begin{array}{rcl}
4x^2 + 8x &amp; = &amp; 4x(x + 2)
\end{array}
        </me>
      </solution>
    </example>

    <example>
      <statement>
        <p>
          Factor <m>-3x^3 + 6x^2</m>.
        </p>
      </statement>
      <solution>
        <p>
          Both terms share a factor of <m>3x^2</m>.
          Factoring out a negative sign is often helpful.
        </p>
        <me>
\begin{array}{rcl}
-3x^3 + 6x^2 &amp; = &amp; -3x^2(x - 2)
\end{array}
        </me>
      </solution>
    </example>

    <remark>
      <p>
        Always check for a greatest common factor first.
        Many factoring mistakes come from skipping this step.
      </p>
    </remark>
  </subsection>

  <!-- ======================================================= -->
  <subsection xml:id="ssec-factor-difference-squares">
    <title>Difference of Squares</title>

    <p>
      One of the most common factoring patterns is the difference of squares.
      This pattern appears frequently in limits and rational expressions.
    </p>

    <principle xml:id="pr-difference-squares">
      <statement>
        <me>
\begin{array}{rcl}
a^2 - b^2 &amp; = &amp; (a - b)(a + b)
\end{array}
        </me>
      </statement>
    </principle>

    <example>
      <statement>
        <p>
          Factor <m>x^2 - 16</m>.
        </p>
      </statement>
      <solution>
        <p>
          Recognize <m>16 = 4^2</m>.
        </p>
        <me>
\begin{array}{rcl}
x^2 - 16 &amp; = &amp; (x - 4)(x + 4)
\end{array}
        </me>
      </solution>
    </example>

    <example>
      <statement>
        <p>
          Factor <m>9x^2 - 25</m>.
        </p>
      </statement>
      <solution>
        <p>
          Rewrite each term as a square.
        </p>
        <me>
\begin{array}{rcl}
9x^2 - 25 &amp; = &amp; (3x)^2 - 5^2 \\
          &amp; = &amp; (3x - 5)(3x + 5)
\end{array}
        </me>
      </solution>
    </example>

    <remark>
      <p>
        The sum of squares <m>a^2 + b^2</m> does not factor over the real numbers.
      </p>
    </remark>
  </subsection>

  <!-- ======================================================= -->
  <subsection xml:id="ssec-factor-perfect-squares">
    <title>Perfect Square Trinomials</title>

    <p>
      Some trinomials arise from squaring a binomial.
      Recognizing these patterns allows quick factoring.
    </p>

    <principle xml:id="pr-perfect-square">
      <statement>
        <me>
\begin{array}{rcl}
a^2 + 2ab + b^2 &amp; = &amp; (a + b)^2 \\[0.6em]
a^2 - 2ab + b^2 &amp; = &amp; (a - b)^2
\end{array}
        </me>
      </statement>
    </principle>

    <example>
      <statement>
        <p>
          Factor <m>x^2 + 6x + 9</m>.
        </p>
      </statement>
      <solution>
        <p>
          The middle term matches <m>2ab</m> with <m>a = x</m> and <m>b = 3</m>.
        </p>
        <me>
\begin{array}{rcl}
x^2 + 6x + 9 &amp; = &amp; (x + 3)^2
\end{array}
        </me>
      </solution>
    </example>

    <example>
      <statement>
        <p>
          Factor <m>x^2 - 10x + 25</m>.
        </p>
      </statement>
      <solution>
        <me>
\begin{array}{rcl}
x^2 - 10x + 25 &amp; = &amp; (x - 5)^2
\end{array}
        </me>
      </solution>
    </example>
  </subsection>

  <!-- ======================================================= -->
  <subsection xml:id="ssec-factor-general-trinomials">
    <title>Factoring General Trinomials</title>

    <p>
      Not all trinomials are perfect squares.
      For expressions of the form <m>x^2 + bx + c</m>,
      we look for two numbers whose product is <m>c</m>
      and whose sum is <m>b</m>.
    </p>

    <example>
      <statement>
        <p>
          Factor <m>x^2 + 5x + 6</m>.
        </p>
      </statement>
      <solution>
        <p>
          We need two numbers that multiply to <m>6</m>
          and add to <m>5</m>.
        </p>
        <me>
\begin{array}{rcl}
x^2 + 5x + 6 &amp; = &amp; (x + 2)(x + 3)
\end{array}
        </me>
      </solution>
    </example>

    <example>
      <statement>
        <p>
          Factor <m>x^2 - x - 12</m>.
        </p>
      </statement>
      <solution>
        <p>
          The product is <m>-12</m> and the sum is <m>-1</m>.
        </p>
        <me>
\begin{array}{rcl}
x^2 - x - 12 &amp; = &amp; (x - 4)(x + 3)
\end{array}
        </me>
      </solution>
    </example>
  </subsection>

  <!-- ======================================================= -->
  <subsection xml:id="ssec-factor-importance-calculus">
    <title>Why Factoring Matters in Calculus</title>

    <p>
      In calculus, factoring is often used to cancel terms
      before evaluating a limit.
      Expressions that initially appear undefined can often
      be simplified using factoring.
    </p>

    <example>
      <statement>
        <p>
          Simplify <m>\dfrac{x^2 - 9}{x - 3}</m> for <m>x \neq 3</m>.
        </p>
      </statement>
      <solution>
        <p>
          Factor the numerator.
        </p>
        <me>
\begin{array}{rcl}
\dfrac{x^2 - 9}{x - 3}
&amp; = &amp;
\dfrac{(x - 3)(x + 3)}{x - 3} \\[0.6em]
&amp; = &amp;
x + 3
\end{array}
        </me>
      </solution>
    </example>

    <remark>
      <p>
        This exact type of simplification appears repeatedly in limit problems.
      </p>
    </remark>
  </subsection>

</section>
