<?xml version="1.0" encoding="UTF-8"?>

<section xml:id="sec-precalc-exp" xmlns:xi="http://www.w3.org/2001/XInclude">
  <title>Exponentials</title>

  <p>
    Exponential functions play a central role in calculus.
    They arise in models of population growth, radioactive decay,
    compound interest, and many other applications.
    In this section, we review the algebraic properties of exponents
    and develop systematic methods for solving exponential equations.
  </p>

  <p>
    The focus here is on algebraic techniques.
    Later in the course, these same ideas will be extended using logarithms
    and calculus.
  </p>

  <!-- ======================================================= -->
  <subsection xml:id="ssec-exp-def">
    <title>Exponential Expressions</title>

    <p>
      An exponential expression is one in which the variable appears in the exponent.
      For example, <m>2^x</m> and <m>e^{3x}</m> are exponential expressions.
    </p>

    <definition xml:id="def-exponential-function">
      <title>Exponential Function</title>
      <statement>
        <p>
          An <term>exponential function</term> is a function of the form
        </p>
        <me>
          f(x) = a^x,
        </me>
        <p>
          where <m>a &gt; 0</m> and <m>a \neq 1</m>.
        </p>
      </statement>
    </definition>
  </subsection>

  <!-- ======================================================= -->
  <subsection xml:id="ssec-exp-properties">
    <title>Properties of Exponents</title>

    <p>
      Solving exponential equations relies on the fundamental properties of exponents.
      These rules allow us to rewrite expressions in simpler or more useful forms.
    </p>

    <principle xml:id="pr-exp-laws">
      <statement>
        <p>
          Assume <m>a &gt; 0</m> and <m>m,n</m> are real numbers.
          Then the following properties hold:
        </p>

        <me>
\begin{array}{rcl|rcl}
a^m a^n &amp; = &amp; a^{m+n}, &amp;
\dfrac{a^m}{a^n} &amp; = &amp; a^{m-n} \\[0.6em]
(a^m)^n &amp; = &amp; a^{mn}, &amp;
(ab)^n &amp; = &amp; a^n b^n \\[0.6em]
a^0 &amp; = &amp; 1, &amp;
a^{-n} &amp; = &amp; \dfrac{1}{a^n}
\end{array}
        </me>
      </statement>
    </principle>

    <remark>
      <p>
        These properties do not apply when adding or subtracting exponential terms.
        For example, <m>a^x + a^x \neq a^{2x}</m>.
      </p>
    </remark>
  </subsection>

<!-- ======================================================= -->
<subsection xml:id="ssec-exp-change-base">
  <title>Changing the Base and the Role of <m>e</m></title>

  <p>
    In algebra, exponential expressions can be written using many different bases.
    In calculus, however, it is often convenient to rewrite exponentials
    using base <m>e</m>.
    This is because derivatives and integrals involving <m>e^x</m>
    have especially simple formulas.
  </p>

  <p>
    The idea of <em>changing the base</em> allows us to rewrite
    any exponential expression in terms of a different base.
    Later, logarithms will give us a systematic way to do this.
  </p>

  <principle xml:id="pr-exp-change-base">
    <statement>
      <p>
        Any exponential expression <m>a^x</m> with <m>a &gt; 0</m> and <m>a \neq 1</m>
        can be rewritten using base <m>e</m>.
      </p>
      <p>
        In particular, there exists a real number <m>k</m> such that
      </p>
      <me>
        a^x = e^{kx}.
      </me>
    </statement>
  </principle>

  <remark>
    <p>
      The value of <m>k</m> depends on the base <m>a</m>.
      Later in the course, we will see that <m>k = \ln(a)</m>,
      where <m>\ln</m> is the natural logarithm.
    </p>
  </remark>

  <example>
    <statement>
      <p>
        Rewrite <m>2^x</m> using base <m>e</m>.
      </p>
    </statement>
    <solution>
      <p>
        There exists a constant <m>k</m> such that
      </p>
      <me>
        2^x = e^{kx}.
      </me>
      <p>
        This constant is <m>k = \ln(2)</m>, so
      </p>
      <me>
        2^x = e^{(\ln 2)x}.
      </me>
    </solution>
  </example>

  <example>
    <statement>
      <p>
        Rewrite <m>5^{3x}</m> using base <m>e</m>.
      </p>
    </statement>
    <solution>
      <p>
        Using the change of base idea,
      </p>
      <me>
        5^{3x} = e^{(\ln 5)(3x)} = e^{3(\ln 5)x}.
      </me>
    </solution>
  </example>

  <remark>
    <p>
      In calculus, derivatives and integrals of <m>e^x</m>
      are much simpler than those of <m>a^x</m> for other bases.
      For this reason, exponential models are often rewritten
      using base <m>e</m> before applying calculus techniques.
    </p>
  </remark>
</subsection>



  <!-- ======================================================= -->
  <subsection xml:id="ssec-exp-eq-same-base">
    <title>Solving Exponential Equations with the Same Base</title>

    <p>
      The simplest exponential equations are those in which both sides
      can be written using the same base.
      In this case, the exponents can be set equal.
    </p>

    <principle xml:id="pr-exp-equal-bases">
      <statement>
        <p>
          If <m>a &gt; 0</m>, <m>a \neq 1</m>, and
        </p>
        <me>
          a^u = a^v,
        </me>
        <p>
          then <m>u = v</m>.
        </p>
      </statement>
    </principle>

    <example>
      <statement>
        <p>
          Solve <m>2^{x+1} = 16</m>.
        </p>
      </statement>
      <solution>
        <p>
          Rewrite both sides with base <m>2</m>.
        </p>

        <me>
\begin{array}{rcl}
2^{x+1} &amp; = &amp; 2^4
\end{array}
        </me>

        <p>
          Set the exponents equal.
        </p>

        <me>
\begin{array}{rcl}
x + 1 &amp; = &amp; 4 \\
x &amp; = &amp; 3
\end{array}
        </me>
      </solution>
    </example>

    <example>
      <statement>
        <p>
          Solve <m>3^{2x-1} = 9</m>.
        </p>
      </statement>
      <solution>
        <p>
          Rewrite <m>9</m> using base <m>3</m>.
        </p>

        <me>
\begin{array}{rcl}
3^{2x-1} &amp; = &amp; 3^2
\end{array}
        </me>

        <p>
          Set exponents equal.
        </p>

        <me>
\begin{array}{rcl}
2x - 1 &amp; = &amp; 2 \\
2x &amp; = &amp; 3 \\
x &amp; = &amp; \dfrac{3}{2}
\end{array}
        </me>
      </solution>
    </example>
  </subsection>

  <!-- ======================================================= -->
  <subsection xml:id="ssec-exp-eq-rewrite">
    <title>Solving Exponential Equations by Rewriting</title>

    <p>
      Sometimes an equation does not initially have matching bases.
      In these cases, we attempt to rewrite both sides using a common base.
    </p>

    <example>
      <statement>
        <p>
          Solve <m>4^x = 2^{x+3}</m>.
        </p>
      </statement>
      <solution>
        <p>
          Rewrite <m>4</m> as a power of <m>2</m>.
        </p>

        <me>
\begin{array}{rcl}
(2^2)^x &amp; = &amp; 2^{x+3}
\end{array}
        </me>

        <p>
          Simplify and equate exponents.
        </p>

        <me>
\begin{array}{rcl}
2^{2x} &amp; = &amp; 2^{x+3} \\
2x &amp; = &amp; x + 3 \\
x &amp; = &amp; 3
\end{array}
        </me>
      </solution>
    </example>
  </subsection>

  <!-- ======================================================= -->
  <subsection xml:id="ssec-exp-no-solution">
    <title>When Exponential Equations Have No Solution</title>

    <p>
      Exponential functions, <m>a^x</m>, are always positive.
      This observation can be used to identify equations with no real solution.
    </p>

    <example>
      <statement>
        <p>
          Solve <m>2^x = -4</m>.
        </p>
      </statement>
      <solution>
        <p>
          Since <m>2^x &gt; 0</m> for all real <m>x</m>,
          this equation has no real solution.
        </p>
      </solution>
    </example>
  </subsection>



</section>
