<?xml version="1.0" encoding="UTF-8"?>

<section xml:id="sec-precalc-funcs" xmlns:xi="http://www.w3.org/2001/XInclude">
  <title>Functions and Inverses</title>

  <p>
   This section reviews functions, function composition, and introduces inverse functions
    from both an algebraic and conceptual perspective.
  </p>

  <!-- ======================================================= -->
  <subsection xml:id="ssec-function-review">
    <title>Functions and Notation</title>

    <p>
      A function assigns exactly one output to each input.
      We typically write a function using function notation,
      such as <m>f(x)</m>.
    </p>

    <definition xml:id="def-function">
      <title>Function</title>
      <statement>
        <p>
          A <term>function</term> is a rule that assigns to each input
          <m>x</m> in its domain exactly one output, denoted <m>f(x)</m>.
        </p>
      </statement>
    </definition>

    <example>
      <statement>
        <p>
          Let <m>f(x) = 2x + 1</m>. Find <m>f(3)</m>.
        </p>
      </statement>
      <solution>
        <me>
\begin{array}{rcl}
f(3) &amp; = &amp; 2(3) + 1 \\
     &amp; = &amp; 7
\end{array}
        </me>
      </solution>
    </example>
  </subsection>

  <!-- ======================================================= -->
  <subsection xml:id="ssec-composition">
    <title>Function Composition</title>

    <p>
      Function composition describes applying one function to the output of another.
      Composition is important because inverse functions are defined
      in terms of composition.
    </p>

    <definition xml:id="def-composition">
      <title>Function Composition</title>
      <statement>
        <p>
          If <m>f</m> and <m>g</m> are functions, the <term>composition</term>
          of <m>f</m> with <m>g</m> is defined by
        </p>
        <me>
          (f \circ g)(x) = f(g(x)).
        </me>
      </statement>
    </definition>

    <example>
      <statement>
        <p>
          Let <m>f(x) = 2x + 1</m> and <m>g(x) = x^2</m>.
          Find <m>(f \circ g)(x)</m>.
        </p>
      </statement>
      <solution>
        <me>
\begin{array}{rcl}
(f \circ g)(x) &amp; = &amp; f(g(x)) \\
               &amp; = &amp; f(x^2) \\
               &amp; = &amp; 2x^2 + 1
\end{array}
        </me>
      </solution>
    </example>

    <remark>
      <p>
        In general, <m>f \circ g</m> and <m>g \circ f</m> are not the same.
      </p>
    </remark>
  </subsection>

  <!-- ======================================================= -->
  <subsection xml:id="ssec-inverses">
    <title>Inverse Functions</title>

    <p>
      An inverse function reverses the action of a function.
      When a function and its inverse are composed,
      the result is the original input.
    </p>

    <definition xml:id="def-inverse-function">
      <title>Inverse Function</title>
      <statement>
        <p>
          A function <m>f</m> has an <term>inverse</term>, denoted <m>f^{-1}</m>,
          if
        </p>
        <me>
\begin{array}{rcl}
f(f^{-1}(x)) &amp; = &amp; x
\quad \text{and} \quad
f^{-1}(f(x)) &amp; = &amp; x.
\end{array}
        </me>
      </statement>
    </definition>

    <remark>
      <p>
        Not every function has an inverse.
        A function must be one-to-one,
        meaning different inputs produce different outputs.
      </p>
    </remark>
  </subsection>

  <!-- ======================================================= -->
  <subsection xml:id="ssec-finding-inverses">
    <title>Finding Inverses Algebraically</title>

    <p>
      To find an inverse function algebraically,
      we solve the equation <m>y = f(x)</m> for <m>x</m>
      and then interchange the roles of <m>x</m> and <m>y</m>.
    </p>

    <example>
      <statement>
        <p>
          Find the inverse of <m>f(x) = 2x + 1</m>.
        </p>
      </statement>
      <solution>
        <p>
          Step 1: Write the equation <m>y = 2x + 1</m>.
        </p>

        <p>
          Step 2: Solve for <m>x</m>.
        </p>

        <me>
\begin{array}{rcl}
y - 1 &amp; = &amp; 2x \\
x &amp; = &amp; \dfrac{y - 1}{2}
\end{array}
        </me>

        <p>
          Step 3: Interchange <m>x</m> and <m>y</m>.
        </p>

        <me>
          f^{-1}(x) = \dfrac{x - 1}{2}.
        </me>
      </solution>
    </example>
  </subsection>

  <!-- ======================================================= -->
  <subsection xml:id="ssec-special-inverses">
    <title>Important Examples of Inverse Functions</title>

    <p>
      Several inverse function pairs appear repeatedly in calculus.
      These relationships are important to recognize and remember.
    </p>

    <example xml:id="ex-precalc-expInv">
      <statement>
        <p>
          The exponential function <m>e^x</m> and the natural logarithm
          <m>\ln(x)</m> are inverses.
        </p>
      </statement>
      <solution>
        <me>
\begin{array}{rcl}
e^{\ln(x)} &amp; = &amp; x \quad (x &gt; 0) \\
\ln(e^x) &amp; = &amp; x
\end{array}
        </me>
      </solution>
    </example>

    <example>
      <statement>
        <p>
          Trigonometric functions also have inverses.
          For example, <m>\sin(x)</m> and <m>\arcsin(x)</m> are inverse functions
          when appropriate domain restrictions are used.
        </p>
      </statement>
      <solution>
        <me>
\begin{array}{rcl}
\sin(\arcsin(x)) &amp; = &amp; x \quad (-1 \le x \le 1) \\
\arcsin(\sin(x)) &amp; = &amp; x \quad \left(-\dfrac{\pi}{2} \le x \le \dfrac{\pi}{2}\right)
\end{array}
        </me>
      </solution>
    </example>

    <remark>
      <p>
        Inverse trigonometric functions require restricted domains
        so that they are one-to-one.
      </p>
    </remark>
  </subsection>


</section>
