<?xml version="1.0" encoding="UTF-8"?>
<section xmlns:xi="http://www.w3.org/2001/XInclude" xml:lang="en-US" xml:id="sec-limit-ww">
  <title>Additional Worked-Out Problems</title>
    <subsection xml:id="subsec-limit-gl">
      <title><xref ref="sec-graphical-limits"/> Limits from Graphs and Notation</title>
      
      <example xml:id="ex-limit-graph-02">
        <title>Graphing a Function to Find a Limit</title>
        <statement>
          <p>
            Consider the function <m>f(x) = \begin{cases} x^2 &amp; \text{ if } x \lt 2 \\ 3 &amp; \text{ if } x = 2 \\ 4 - x &amp; \text{ if } x \gt 2 \end{cases}</m>. 
          </p>
          <p> Sketch the graph of <m>f</m> and use it to find <m>\displaystyle\lim_{x \to 2} f(x)</m>, if it exists.
          </p>
        </statement>
        <solution>
          <p>
            To graph <m>f</m>, we first graph the pieces of the function on their respective domains. For <m>x \lt 2</m>, we graph <m>y = x^2</m>, 
            which is a parabola opening upwards. At <m>x = 2</m>, we have a single point <m>(2, 3)</m>. For <m>x \gt 2</m>, we graph <m>y = 4 - x</m>, 
            which is a line with a negative slope. Together, these pieces form the graph of <m>f</m>.
          </p>
          <p> 
<figure xml:id="fig-limit-piecewise-02">
  <caption>
    Graph of a piecewise-defined function <m>f(x)</m> as described in the example.
  </caption>
  <image source="images/limitFunc02.PNG" width="100%">
    <shortdescription>
      A graph on a coordinate grid showing a piecewise function.
      For x less than 2, the graph is a smooth upward-opening curve with a minimum at the origin.
      As x approaches 2 from the left, the curve rises toward an open circle at x equals 2 and height 4.
      At x equals 2, there is a filled point at height 3, indicating the function value.
      Also at x equals 2, there is an open circle at height 2 that begins a straight line segment.
      For x greater than 2, the graph is a straight line sloping downward from the open circle at x equals 2 and height 2,
      passing through the point x equals 3 and height 1, and continuing downward toward x equals 4.
      The differing open and closed points at x equals 2 show that the left-hand limit, right-hand limit,
      and the function value at x equals 2 are not all the same.
    </shortdescription>
  </image>
</figure>
          </p>
          <p> Now, we analyze the behavior of <m>f(x)</m> as <m>x</m> approaches 2 from both sides. 
            As <m>x</m> approaches 2 from the left (<m>x \to 2^-</m>), <m>f(x) = x^2</m> approaches <m>4</m>. 
            As <m>x</m> approaches 2 from the right (<m>x \to 2^+</m>), <m>f(x) = 4 - x</m> approaches <m>2</m>.
          </p>
          <p> Since the left-hand limit (<m>4</m>) and the right-hand limit (<m>2</m>) are not equal, the overall limit <m>\displaystyle\lim_{x \to 2} f(x)</m> does not exist.
          </p>
          
        </solution>

      </example>

<example xml:id="ex-vert-asymptotes-rational-01">
  <statement>
    <p>
      Consider the function
      <m>\displaystyle f(x)=\frac{x^2-1}{x^2+3x+2}</m>.
    </p> 
        <p>
          Find all the vertical asymptotes of <m>f</m>.
        </p>
  </statement>
  <solution>
    <p>
      To find the vertical asymptotes of the function <m>f(x)=\frac{x^2-1}{x^2+3x+2}</m>, we first factor the denominator:
      <m>x^2 + 3x + 2 = (x + 1)(x + 2)</m>.
      The vertical asymptotes occur where the denominator is zero, provided the numerator is not also zero at those points.
      Setting the denominator equal to zero gives us:
      <m>(x + 1)(x + 2) = 0</m>,
      which has solutions <m>x = -1</m> and <m>x = -2</m>. </p> <p> 
      Next, we check the numerator at these points:
      <m>x^2 - 1 = (x - 1)(x + 1)</m>. </p> <p> 
      At <m>x = -1</m>, the numerator is zero, indicating there is no vertical asymptote there (in fact it will be called a removable discontinuity once we learn
      about this in our continuity section). </p><p>
      At <m>x = -2</m>, the numerator is non-zero (<m>3</m>), confirming that there is a vertical asymptote at this point. </p><p>
      Therefore, the only vertical asymptote of <m>f</m> is at <m>x = -2</m>.
    </p>
  </solution>
</example>


    </subsection>

    <subsection xml:id="subsec-limit-alg">
      <title><xref ref="sec-limit-laws"/> Limit Laws and Algebraic Techniques</title>

      <example xml:id="ex-limit-rational-a-zero-01">
  <statement>
    <p>
      Evaluate the limit: 
    <m>
      \displaystyle \lim_{a \to 0} \frac{(a-3)^2 - 9}{a}.
    </m>
    </p>
  </statement>

  <solution>
    <p>
      Begin by simplifying the expression in the numerator.
      Expand <m>(a-3)^2</m>:
    </p>

    <me>
\begin{array}{rcl}
(a-3)^2 - 9
&amp; =&amp;  (a^2 - 6a + 9) - 9 \\
&amp;=&amp; a^2 - 6a.
\end{array}
    </me>

    <p>
      Substituting this back into the limit gives
    </p>

    <me>
      \displaystyle \lim_{a \to 0} \frac{a^2 - 6a}{a}.
    </me>

    <p>
      Factor <m>a</m> from the numerator and simplify:
    </p>

    <me>
\begin{array}{rcl}
\displaystyle \lim_{a \to 0} \frac{a(a-6)}{a}
&amp; =&amp; \displaystyle \lim_{a \to 0} (a-6).
\end{array}
    </me>

    <p>
      Now evaluate the limit by direct substitution:
    </p>

    <me>
      \displaystyle \lim_{a \to 0} (a-6) = -6.
    </me>

    <p>
      Therefore, the value of the limit is <m>-6</m>.
    </p>
  </solution>
</example>

<example xml:id="ex-limit-difference-quotient-01">
  <statement>
    <p>
      Evaluate the limit: 
    <m>
      \displaystyle \lim_{h \to 1} \frac{\frac{1}{h+1} - \frac{1}{2}}{h-1}.
    </m>
        </p>
  </statement>

  <solution>
    <p>
      Direct substitution gives a meaningless expression <m>\frac{0}{0}</m>,
      so we begin by simplifying the numerator.
    </p>

    <p>
      Combine the fractions in the numerator using a common denominator:
    </p>

    <me>
\begin{array}{rcl}
\displaystyle \frac{1}{h+1} - \frac{1}{2}
&amp; =&amp; \displaystyle \frac{2 - (h+1)}{2(h+1)}.
\end{array}
    </me>

    <p>
      Simplify the numerator:
    </p>

    <me>
2 - (h+1) = 1 - h.
    </me>

    <p>
      Substitute this back into the original expression:
    </p>

    <me>
 \frac{\frac{1}{h+1} - \frac{1}{2}}{h-1}
= \frac{1-h}{2(h+1)(h-1)}.

    </me>

    <p>
      Notice that <m>1-h = -(h-1)</m>, so we can factor and cancel:
    </p>

    <me>
\begin{array}{rcl}
\displaystyle \frac{1-h}{2(h+1)(h-1)}
&amp;=&amp; \displaystyle \frac{-(h-1)}{2(h+1)(h-1)}
\\[0.8em]
&amp;=&amp; \displaystyle -\frac{1}{2(h+1)}.
\end{array}
    </me>

    <p>
      Now we can safely evaluate the limit by substitution:
    </p>

    <me>
      \displaystyle \lim_{h \to 1} -\frac{1}{2(h+1)} = -\frac{1}{4}.
    </me>

    <p>
      Therefore,
    </p>

    <me>
      \displaystyle \lim_{h \to 1} \frac{\frac{1}{h+1} - \frac{1}{2}}{h-1} = -\frac{1}{4}.
    </me>
  </solution>
</example>

<example xml:id="ex-squeeze-x-2-cos-poly">
  <statement>
    <p>
      Suppose <m>f</m> is a function such that for all <m>x</m>,
    </p>
    <me>
      \cos(\pi x)\le f(x)\le x^2-4x+5.
    </me>
    <p>
      Use the Squeeze Theorem to evaluate <m>\displaystyle \lim_{x\to 2} f(x)</m>, or explain why the Squeeze Theorem does not apply.
    </p>
  </statement>

  <solution>
    <p>
      Compute the limits of the bounding functions as <m>x\to 2</m>.
      Since <m>\cos(\pi x)</m> and polynomials are continuous, we can substitute <m>x=2</m>:
    </p>

    <me>
\begin{array}{rcl}
\displaystyle \lim_{x\to 2}\cos(\pi x)
&amp;=&amp; \cos(2\pi)=1,
\\[0.8em]
\displaystyle \lim_{x\to 2}(x^2-4x+5)
&amp;=&amp; 2^2-4(2)+5
\\[0.4em]
&amp;=&amp; 4-8+5
\\[0.4em]
&amp;=&amp; 1.
\end{array}
    </me>

    <p>
      Both bounding functions approach the same value, <m>1</m>. Therefore, by the Squeeze Theorem,
    </p>

    <me>
      \displaystyle \lim_{x\to 2} f(x)=1.
    </me>
  </solution>
</example>



    </subsection>


    <subsection xml:id="subsec-limit-inf">
      <title><xref ref="sec-limit-inf"/> Limits at Infinity: Horizontal Asymptotes</title>

      
<example xml:id="ex-limit-infinity-radical-rational">
  <statement>
    <p>
      Evaluate the limit: 
    <m>
      \displaystyle \lim_{x\to\infty}
      \frac{\sqrt{x}-x^{-1}}{x^{3/2}-\sqrt[3]{x}}.
    </m>
      </p>
  </statement>

  <solution>
    <p>
      To evaluate this limit, we compare the dominant powers of <m>x</m> in the numerator and denominator.
      The largest power of <m>x</m> in the numerator is <m>x^{1/2}</m>, and the largest power of <m>x</m> in the denominator is <m>x^{3/2}</m>. Therefore
    </p>

    <me>
      f(x) \approx \frac{x^{1/2}}{x^{3/2}} = x^{-1} = \frac{1}{x}.
    </me>

    <p>
      As <m>x \to \infty</m>, <m>\frac{1}{x} \to 0</m>. Thus, the limit is 
    </p>

    <me>
      \displaystyle \lim_{x\to\infty}
      \frac{\sqrt{x}-x^{-1}}{x^{3/2}-\sqrt[3]{x}} = 0.
    </me>
  </solution>
</example>

<example xml:id="ex-limit-infinity-polynomial-dominant">
  <statement>
    <p>
      Evaluate the limits
    </p>
    <me>
      \displaystyle 
      \lim_{x\to\infty}\frac{3-2x-8x^3+3x^4}{2x^4+x+1}
      \quad\text{and}\quad
      \lim_{x\to -\infty}\frac{3-2x-8x^3+3x^4}{2x^4+x+1}.
    </me>
  </statement>

  <solution>
    <p>
      To evaluate limits at infinity for rational functions, we compare the dominant (highest–power) terms
      in the numerator and denominator.
      In this case, the dominant term in the numerator is <m>3x^4</m>, and the dominant term in the denominator
      is <m>2x^4</m>.
    </p>

    <p>
      For large values of <m>|x|</m>, the lower–degree terms become negligible, so the function behaves like
    </p>

    <me>
      f(x) \approx \frac{3x^4}{2x^4} = \frac{3}{2}.
    </me>

    <p>
      Since both dominant terms involve <m>x^4</m>, which is positive for both positive and negative values of <m>x</m>,
      this approximation applies as <m>x\to\infty</m> and as <m>x\to -\infty</m>.
    </p>

    <me>
      \displaystyle 
      \lim_{x\to\infty}\frac{3-2x-8x^3+3x^4}{2x^4+x+1}
      =
      \lim_{x\to -\infty}\frac{3-2x-8x^3+3x^4}{2x^4+x+1}
      =
      \frac{3}{2}.
    </me>
  </solution>
</example>


<example xml:id="ex-limit-infinity-horizontal-asymptote-sqrt-x2plus1">
  <statement>
    <p>
      Let <m>f(x)=\dfrac{\sqrt{x^{2}+1}}{x+1}</m>.
    </p>
    <p>
      (a) Evaluate <m>\displaystyle \lim_{x\to\infty} f(x)</m>. </p><p>
      (b) Find the equation of the horizontal asymptote associated with this limit.
    </p>
  </statement>

  <solution>
    <p>
      (a) To evaluate <m>\displaystyle \lim_{x\to\infty} f(x)</m>, we analyze the dominant terms in the numerator and denominator.
      The dominant term in the numerator is <m>\sqrt{x^{2}} = x</m>, and the dominant term in the denominator is <m>x</m>.
      Therefore, for large values of <m>|x|</m>, the function behaves like
    </p>
    <me>
      f(x) \approx \frac{x}{x} = 1.
    </me>
    <p>
      Thus,
    </p>
    <me>
      \displaystyle \lim_{x\to\infty} f(x) = 1.
    </me>

    <p>
      (b) Since <m>\displaystyle \lim_{x\to\infty} f(x)=1</m>, the curve approaches height <m>1</m> as <m>x</m> becomes large.
      Therefore the horizontal asymptote (for <m>x\to\infty</m>) is
      <m>y=1</m>.
    </p>
  </solution>
</example>


<example xml:id="ex-limit-infinity-sqrt-minus-x">
  <statement>
    <p>
      Evaluate the limit: 
  <m>
      \displaystyle \lim_{x\to\infty} \left(\sqrt{x^2+x}-x\right).
    </m>
    </p>
  </statement>

  <solution>
    <p>
      Direct substitution leads to a confusing expression of the form <m>\infty-\infty</m>.
      To resolve this and apply our technique, let's first multiply by the conjugate of the expression.
    </p>

     <me>
\begin{array}{rcl}
\displaystyle \sqrt{x^2+x}-x
\amp=\amp \displaystyle \left(\sqrt{x^2+x}-x\right)
\cdot \frac{\sqrt{x^2+x}+x}{\sqrt{x^2+x}+x}
\\[1.2em]
\amp=\amp \displaystyle \frac{(x^2+x)-x^2}{\sqrt{x^2+x}+x}
\\[1.2em]
\amp=\amp \displaystyle \frac{x}{\sqrt{x^2+x}+x}.
\end{array}
    </me>

   <p>The dominant term in the numerator is <m>x</m>, and the dominant term in the denominator is also <m>x</m>.
   Therefore, for large values of <m>\sqrt{x^2} = x</m>, the function behaves like</p>
    <me>
      f(x) \approx \frac{x}{\sqrt{x^2} + x} = \frac{x}{x+x} = \frac{1}{2}. 
    </me>
    

    <p>
      Thus,
    </p>
    <me>
      \displaystyle \lim_{x\to\infty} \left(\sqrt{x^2+x}-x\right) = \frac{1}{2}.
    </me>

  </solution>
</example>


    </subsection>

    <subsection xml:id="subsec-limit-cont">
      <title><xref ref="sec-limit-continuity"/> Continuity</title>

      
<example xml:id="ex-continuity-realworld-02">
  <statement>
    <p>
      For each function defined below, determine whether it is <em>continuous</em> or <em>discontinuous</em>.
      Briefly justify your choice.
    </p>


        <p>
          (a) Let <m>f(t)</m> be the amount of water (in gallons) remaining in a reservoir after <m>t</m> hours of steady drainage.
</p>
        <p>
          (b) Let <m>g(t)</m> be the floor number that an elevator is on at time <m>t</m> seconds.
        </p>

        <p>
          (c) Let <m>h(d)</m> be the number of pages read in a book after <m>d</m> days.
        </p>

  </statement>
  <solution>
    <p>
      (a) <alert>Continuous</alert>. The function <m>f(t)</m> is continuous because the amount of water in the reservoir changes smoothly over time as it drains steadily.
      There are no sudden jumps or breaks in the amount of water; it decreases gradually.
    </p>
    <p>
      (b) <alert>Discontinuous</alert>. The function <m>g(t)</m> is discontinuous because the elevator moves between floors in jumps.
      The floor number changes suddenly when the elevator passes from one floor to the next.
    </p>
    <p>
      (c) <alert>Discontinuous</alert>. The function <m>h(d)</m> is discontinuous because the number of pages read is a step function.
      The number of pages read increases in whole numbers, resulting in jumps rather than a smooth change
    </p>
  </solution>
</example>


<example xml:id="ex-continuity-removable-02">
  <title>Assessing and Fixing a Removable Discontinuity</title>

  <statement>
    <p>
      Let
    </p> <p> 
    <me>
      f(x)=
      \begin{cases}
        \dfrac{x-2}{x^2+3x-10}, &amp; x \neq 2,\\[0.6em]
        4, &amp; x = 2.
      \end{cases}
    </me>
</p> <p>
      (a) Determine whether <m>f</m> is continuous at <m>x=2</m>. Justify your answer.
    </p> <p>
      (b) If <m>f</m> is not continuous at <m>x=2</m>, explain how to redefine <m>f(2)</m> so that <m>f</m> becomes continuous at <m>x=2</m>.
    </p> 
  </statement>

  <solution>
    <p>
      (a) To evaluate the limit as <m>x \to 2</m>, we first simplify the expression for <m>x \neq 2</m>.
      Factor the denominator:
    </p>

    <me>
      x^2 + 3x - 10 = (x+5)(x-2).
    </me>

    <p>
      For <m>x \neq 2</m>, the function simplifies to
    </p>

    <me>
      f(x) = \frac{x-2}{(x+5)(x-2)} = \frac{1}{x+5}.
    </me>

    <p>
      Therefore,
    </p>

    <me>
      \lim_{x\to 2} f(x) = \frac{1}{2+5} = \frac{1}{7}.
    </me>

    <p>
      However, the value of the function at <m>x=2</m> is
      <m> f(2) = 4.
    </m>
      Since the limit exists but is not equal to the function value,
      <m>f</m> is <em>not continuous</em> at <m>x=2</m>.
      This is a <term>removable discontinuity</term>.
    </p>

    <p>
     (b) To remove the discontinuity, we redefine <m>f(2)</m> to equal the limit:
    </p>

    <me>
      f(2) = \frac{1}{7}.
    </me>

    <p>
      With this definition, <m>f</m> becomes continuous at <m>x=2</m>. The full definition of <m>f</m> is now
    </p>
    <me>
      f(x)=
      \begin{cases}
        \dfrac{x-2}{x^2+3x-10}, &amp; x \neq 2,\\[0.6em]
        \dfrac{1}{7}, &amp; x = 2.
      \end{cases}
    </me>

  </solution>
</example>

<example xml:id="ex-classify-discontinuities-graph">
  <introduction>
    <p>
      The graph of a function <m>f</m> is shown in the figure below.</p>
      <figure xml:id="fig-discontinuous-piecewise">
  <caption>
    Graph of a piecewise-defined function illustrating several types of discontinuities,
  </caption>

  <image source="images/discont01.png" width="85%">
    <shortdescription>
      A graph of a function on a coordinate grid.
      On the left, a smooth increasing curve approaches the point (0, 2) but has an open circle there.
      At x = 0, the function instead has a filled point at (0, -1), indicating a jump.
      From x = 0 to x = 1, a straight line rises from (0, -1) to an open circle at (1, 1).
      From x = 1 to x = 3, a straight line descends from the open circle at (1, 1) to a filled point at (3, -1).
      A dashed vertical line at x = 3 indicates a vertical asymptote.
      For x greater than 3, the graph shows a decreasing curve that approaches the asymptote from the right
      and decreases toward zero as x increases.
    </shortdescription>
  </image>
</figure>
<p> 
      For each value of <m>x</m> listed below, determine whether <m>f</m> is continuous or discontinuous at that point.
      If <m>f</m> is discontinuous, classify the type of discontinuity.
    </p>
  </introduction>

  <task>
    <statement>
      <p>
        Classify the behavior of <m>f</m> at <m>x=0</m>.
      </p>
    </statement>
    <solution>
      <p>
        From the graph, as <m>x \to 0^-</m>, the function approaches the open circle at height <m>2</m>,
        while as <m>x \to 0^+</m>, the function approaches the value <m>-1</m>.
        Since the one-sided limits are not equal, the limit does not exist.
      </p>
      <p>
        Therefore, <m>f</m> has a <term>jump discontinuity</term> at <m>x=0</m>.
      </p>
    </solution>
  </task>

  <task>
    <statement>
      <p>
        Classify the behavior of <m>f</m> at <m>x=1</m>.
      </p>
    </statement>
    <solution>
      <p>
        As <m>x \to 1</m> from both sides, the graph approaches the same height,
        indicated by an open circle at <m>(1,1)</m>.
        However, there is no filled point at <m>x=1</m>, so <m>f(1)</m> is not defined.
      </p>
      <p>
        Since the limit exists but <m>f(1)</m> is undefined, <m>f</m> has a
        <term>removable discontinuity</term> at <m>x=1</m>.
      </p>
    </solution>
  </task>

  <task>
    <statement>
      <p>
        Classify the behavior of <m>f</m> at <m>x=3</m>.
      </p>
    </statement>
    <solution>
      <p>
        The graph shows a dashed vertical line at <m>x=3</m>, and the function values increase without bound
        as <m>x \to 3^+</m>.
        This indicates that the function grows arbitrarily large near <m>x=3</m>.
      </p>
      <p>
        Therefore, <m>f</m> has an <term>infinite discontinuity</term>
        (a vertical asymptote) at <m>x=3</m>.
      </p>
    </solution>
  </task>

  <task>
    <statement>
      <p>
        On which intervals shown in the graph is <m>f</m> continuous?
      </p>
    </statement>
    <solution>
      <p>
        The function is continuous on any interval that does not include a discontinuity.
        From the graph, <m>f</m> is continuous on
      </p>
      <me>
        (-\infty,0)\cup(0,1)\cup(1,3)\cup(3,\infty).
      </me>
    </solution>
  </task>
</example>



    </subsection>

    <subsection xml:id="subsec-limit-ivt">
      <title><xref ref="sec-limit-ivt"/> Intermediate Value Theorem</title>

      
  <example xml:id="ivt-04">
    <statement>
      <p>
        A function <m>f</m> is continuous on <m>[2,5]</m>, with <m>f(2)=7</m> and <m>f(5)=1</m>.
        What does the Intermediate Value Theorem guarantee about the equation <m>f(x)=4</m>?
      </p>
    </statement>
  <solution>
    <p>
      Since <m>f</m> is continuous on the interval <m>[2,5]</m> and <m>f(2)=7</m> and <m>f(5)=1</m>,
      the Intermediate Value Theorem states that for any value <m>k</m> between <m>f(2)</m> and <m>f(5)</m>,
      there exists at least one <m>c</m> in <m>(2,5)</m> such that <m>f(c)=k</m>.
      Since <m>4</m> is between <m>7</m> and <m>1</m>, there exists at least one <m>c</m> in <m>(2,5)</m> such that <m>f(c)=4</m>.
    </p>
  </solution>
  </example>
      
  <example xml:id="ivt-02">
    <statement>
      <p>
        Let <m>f(x)=\ln(x)-x+2</m>.
        Use the Intermediate Value Theorem to show that <m>f(x)=0</m> has at least one solution for <m>x&gt;1</m>.
      </p>
    </statement>
  <solution>
    <p>
      First, we need to show that <m>f</m> is continuous for <m>x&gt;1</m>.
      Since <m>\ln(x)</m> and <m>-x+2</m> are both continuous for <m>x&gt;0</m>,
      their sum <m>f(x)=\ln(x)-x+2</m> is also continuous for <m>x&gt;0</m>, and thus for <m>x&gt;1</m>.
    </p>
    <p>
      Next, we evaluate <m>f(1)</m> and <m>f(4)</m>:
    </p>
    <me>
\begin{array}{rcl}
f(1)
&amp;=&amp; \ln(1) - 1 + 2 \\
&amp;=&amp; 0 - 1 + 2 \\
&amp;=&amp; 1,
\\[1em]
f(4)
&amp;=&amp; \ln(4) - 4 + 2 \\
&amp;=&amp; \ln(4) - 2 \lt 0 \quad \text{(since } \ln(4) \lt \ln(e^2)\text{)}.
\end{array}
    </me>
    <p>
      Since <m>f(1)=1&gt;0</m> and <m>f(4)&lt;0</m>, by the Intermediate Value Theorem,
      there exists at least one <m>c</m> in <m>(1,4)</m> such that <m>f(c)=0</m>.
      Therefore, the equation <m>f(x)=0</m> has at least one solution for <m>x&gt;1</m>.
    </p> 

</solution>

  </example>


    <example xml:id="ivt-08">
    <statement>
      <p>
        The temperature <m>T(t)</m> (in degrees Celsius) at a location varies continuously over time.
        If <m>T(8\text{:}00\text{ am})=12</m> and <m>T(2\text{:}00\text{ pm})=26</m>,
        explain why the temperature must have been exactly <m>20^\circ</m> at some time between 8:00 am and 2:00 pm.
      </p>
    </statement>
  <solution>
    <p>
      Since temperature varies continuously over time, the function <m>T(t)</m> is continuous
      on the interval from 8:00 am to 2:00 pm.
      Given that <m>T(8\text{:}00\text{ am})=12</m> and <m>T(2\text{:}00\text{ pm})=26</m>,
      by the Intermediate Value Theorem, for any temperature value <m>k</m> between <m>12</m> and <m>26</m>,  
      there exists at least one time <m>c</m> in the interval from 8:00 am to 2:00 pm such that <m>T(c)=k</m>.
      Since <m>20</m> is between <m>12</m> and <m>26</m>, there must be at least one time <m>c</m> in that interval
      when the temperature was exactly <m>20^\circ</m>.
    </p>
  </solution>
  </example>

    </subsection>



</section>