<?xml version="1.0" encoding="UTF-8"?>
<section xmlns:xi="http://www.w3.org/2001/XInclude" xml:lang="en-US" xml:id="sec-limit-laws">
  <title>Limit Laws and Algebraic Techniques</title>

  <objectives>
    <ul>
      <li>State and apply the basic <term>Limit Laws</term> (sum, difference, constant multiple, product, quotient, power, root).</li>
      <li>Recognize when direct substitution can be used to evaluate a limit and when it leads to meaningless expressions.</li>
      <li>Evaluate limits that initially give meaningless expressions by algebraic manipulation </li>
      <li>Analyze limits of piecewise-defined functions by considering one-sided limits.</li>
      <li>Apply the <term>Squeeze Theorem</term> to evaluate limits of functions bounded above and below.</li>
    </ul>
  </objectives>

  <subsection xml:id="ssec-limit-laws">
    <title>Operations on Limits</title>

    <p>
      Some general combination rules make most limit computations routine. 
    </p>

<theorem xml:id="thm-limit-laws">
<title>Limit Laws</title>
<statement>
<p>
Suppose we know that both <m>\displaystyle \lim_{x\to a} f(x)</m> and <m>\displaystyle \lim_{x\to a} g(x)</m> exist. Then we have the following Limit Laws:
</p>
<ul>
<li><em>Sum:</em> <m>\displaystyle \lim_{x\to a} (f(x) + g(x)) = \lim_{x\to a} f(x) + \lim_{x\to a} g(x)</m>.</li>
<li><em>Difference:</em> <m>\displaystyle \lim_{x\to a} (f(x) - g(x)) = \lim_{x\to a} f(x) - \lim_{x\to a} g(x)</m>.</li>
<li><em>Constant Multiple:</em> <m>\displaystyle \lim_{x\to a} (c f(x)) = c \cdot \lim_{x\to a} f(x)</m>, for a constant <m>c</m>.</li>
<li><em>Product:</em> <m>\displaystyle \lim_{x\to a} f(x) g(x) = (\lim_{x\to a} f(x))(\lim_{x\to a} g(x))</m>.</li>
<li><em>Quotient:</em> <m>\displaystyle \lim_{x\to a} \frac{f(x)}{g(x)} = \frac{\lim_{x\to a} f(x)}{\lim_{x\to a} g(x)}</m>, provided <m>\lim_{x\to a} g(x) \
eq 0</m>.</li>
<li><em>Power:</em> <m>\displaystyle \lim_{x\to a} (f(x))^n = (\lim_{x\to a} f(x))^n</m>, for a whole number <m>n</m>.</li>
<li><em>Root:</em> <m>\displaystyle \lim_{x\to a} \sqrt[n]{f(x)} = \sqrt[n]{\lim_{x\to a} f(x)}</m>, for a whole number<fn>If <m>n</m> is even, we assume <m>\displaystyle\lim_{x\to a} f(x) &gt; 0</m></fn> <m>n</m>.</li>
</ul>
<p>
These all have the form: “The limit of an operation equals the operation applied to the limits.” These Laws are also valid for one-sided limits.
</p>
</statement>
<proof>
<p>
A full proof of these laws requires high-level mathematics and the formal <m>\varepsilon</m>–<m>\delta</m> definition of limits (beyond the scope of this course). 
Rigorous proofs like this can be found in MSU's MTH 320 Real Analysis course. 
For those who would like a glimpse a Real Analysis proof, see <url href="https://www.youtube.com/watch?v=eZ13wOvSg64">this video proving the Limit Sum Law</url> 

</p>
</proof>
</theorem>


<problem xml:id="prob-limit-laws-simple">
<statement>
<p>
Suppose <m>\displaystyle\lim_{x\to 5} f(x) = 2</m> and <m>\displaystyle\lim_{x\to 5} g(x) = 3</m>. Find <m>\displaystyle\lim_{x\to 5} \left(2f(x) - (g(x))^2\right)</m>.
</p>
</statement>
<solution>
<p>
Using the Difference, Constant Multiple, and Power Limit Laws:
</p>
<me>
2\cdot \lim_{x\to 5} f(x) - \left(\lim_{x\to 5} g(x)\right)^2 = 2(2) - (3)^2 = 4 - 9 = -5.
</me>
</solution>
</problem>

  </subsection>

  <subsection xml:id="ssec-plugging-in">
    <title>Limits by Plugging In</title>

    <p>
      Assuming the Limit Laws and the Basic Limits <m>\displaystyle\lim_{x\to a} x = a</m> and <m>\displaystyle\lim_{x\to a} c = c</m>, we can prove that most functions are continuous, meaning the limit can be obtained by direct substitution.
    </p>

    <example xml:id="ex-limit-plug-in">
      <title>A Limit by Substitution</title>
      <statement>
        <p>
          Compute <m>\displaystyle \lim_{x\to 2} \frac{1-\sqrt{x}}{1+x}</m> using the Limit Laws.
        </p>
      </statement>
      <solution>
        <p><alert>Step by Step:</alert></p>
        <me>
          \begin{array}{rcll}
           \displaystyle\lim_{x\to 2} \frac{1-\sqrt{x}}{1+x}
          \amp=\amp 
            \displaystyle\frac{\displaystyle\lim_{x\to 2}\,1{-}\sqrt{x}}{\displaystyle\lim_{x\to 2}\,1+x}
          \amp \text{ by the Quotient Law
          }
          \\[2em]
          \amp=\amp 
            \displaystyle\frac{\displaystyle\lim_{x\to 2}\,1-\displaystyle\lim_{x\to 2}\sqrt{x}}{\displaystyle\lim_{x\to 2}1\,+\,\displaystyle\lim_{x\to 2}x}
          \amp \text{ by the Sum and Difference Laws}\!\!\!
          \\[2em]
          \amp=\amp 
            \displaystyle\frac{\displaystyle\lim_{x\to 2}\,1-\sqrt{\displaystyle\lim_{x\to 2}x}}{\displaystyle\lim_{x\to 2}1\,+\,\displaystyle\lim_{x\to 2}x}
          \amp \text{ by the Root Law}
          \\[2em]
          \amp=\amp 
            \displaystyle\frac{1{-}\sqrt{2}}{1\,{+}\,2}
          \ =\ \frac{1{-}\sqrt{2}}{3}
          \amp \text{ by the Basic Limits.}
          \end{array}
        </me>
        <p>
          Thus the correct limit is obtained simply by substituting <m>x=2</m>.
        </p>
        <p>
          <alert>Note:</alert> The Quotient Law requires that the denominator have a non-zero limit. 
          We tentatively proceed with the computation and find the denominator to be 3, 
          which retrospectively justifies the quotient step.
        </p>
      </solution>
    </example>

    <remark>
      <p>
        Substituting <m>x=a</m> usually gives the correct limit unless it leads to a meaningless expression such as <m>\tfrac{0}{0}</m> or <m>\sqrt{-1}</m> (complex values are not considered in this course).
      </p>
    </remark>

    <p>
      In <xref ref="sec-derivative-trig">Section</xref> and <xref ref="sec-derivative-expChain">Section</xref>, we will verify that trigonometric functions 
 like <m>\sin(x)</m> and <m>\tan(x)</m> are also continuous when defined, 
and the same holds for functions like <m>2^x</m> and <m>\log(x)</m>. 
Thus, this principle works for pretty much all reasonable functions.
    </p>

  </subsection>

  <subsection xml:id="ssec-canceling-zeros">
    <title>Limits by Canceling Zeros</title>

    <p>
      Some of the most important limits are those where substitution gives a meaningless expression like <m>\tfrac{0}{0}</m>. To compute these, we must cancel vanishing factors until the expression can be evaluated.
      This often requires algebraic manipulation such as factoring or multiplying by a conjugate.
    </p>

    <example xml:id="ex-canceling-zeros">
      <title>Canceling Factors</title>
      <statement>
        <p>
          Evaluate <m>\displaystyle \lim_{x\to 2} \frac{x^2-4x+4}{x^2-x-2}</m>.
        </p>
      </statement>
      <solution>
        <p>
          Direct substitution gives the meaningless expression <m>\tfrac{0}{0}</m>, so we must simplify the expression first. Factor numerator and denominator:
        </p>
        <me>
          \begin{array}{rcl}
           \displaystyle\lim_{x\to 2}\frac{(x-2)^2}{(x-2)(x+1)} \amp=\amp \displaystyle\lim_{x\to 2} \frac{x-2}{x+1} \\
          \amp=\amp \frac{0}{3} = 0.
          \end{array}
        </me>

          <remark>
        <p> 
Please note that this example is consistent with what we saw in the previous section. 
Here is a Desmos graph of the function, along with a table of values near <m>x=2</m>. </p>

<url href="https://www.desmos.com/calculator/swij6khoz5"> 
<sidebyside width = "90%">
<figure>
  <caption>
    Graph of <m>f(x)=\dfrac{x^2-4x+4}{x^2-x-2}</m>
  </caption>
  <image width = "100%" source="images/LimitOfFunction01.gif">
  </image>
</figure>
</sidebyside>
</url>

<p> 
Keep in mind, however, that on quizzes and exams you may not have access to a calculator — in those cases the algebraic method will be our primary tool for solving such problems.

 </p>
 </remark>
      </solution>
    </example>

    <example xml:id="ex-conjugate">
      <title>Using a Conjugate</title>
      <statement>
        <p>
          Evaluate <m>\displaystyle \lim_{x\to 9} \frac{x-9}{\sqrt{x}-3}</m>.
        </p>
      </statement>
      <solution>
        <p>
          Direct substitution gives the meaningless expression <m>\tfrac{0}{0}</m>, so we must simplify the expression first. 
        </p>
<p>
  Multiply numerator and denominator by the conjugate <m>\sqrt{x}+3</m>:
</p>
<me>
  \displaystyle\lim_{x\to 9}\frac{x-9}{\sqrt{x}-3}\cdot\frac{\sqrt{x}+3}{\sqrt{x}+3}
  = \lim_{x\to 9}\frac{(x-9)(\sqrt{x}+3)}{(\sqrt{x})^2-3^2}
</me>

<p>
  Simplify the denominator using the difference of squares:
</p>
<me>
  \displaystyle\lim_{x\to 9}\frac{(x-9)(\sqrt{x}+3)}{x-9}
</me>>

<p>
  Now cancel the common factor <m>x-9</m>:
</p>
<me>
  \displaystyle\lim_{x\to 9} (\sqrt{x}+3) = 6.
</me>
  <remark>
<p>
  Again, this algebraic approach is important, but you can also explore the behavior graphically or with tables. 
  View it here: <url href="https://www.desmos.com/calculator/ldglp9hhbw" visual="">Desmos Graph</url>.
</p>
</remark>
      </solution>
    </example>
  </subsection>

  <subsection xml:id="ssec-cases">
    <title>Limits by Cases</title>

    <p>
      Piecewise functions often require evaluating limits separately from the left and right. For example, the absolute value function <m>|x|</m> requires case analysis.
    </p>

    <example xml:id="ex-abs-value">
      <title>Absolute Value Example</title>
      <statement>
        <p>
          Evaluate <m>\displaystyle \lim_{x\to 2} \frac{|x^2-4|}{x-2}</m>.
        </p>
      </statement>
<solution>
  <p>
    We analyze the sign of the expression inside the absolute value. Note that
    <m>x^2 - 4 = (x-2)(x+2)</m>.
  </p>

  <p>
    For <m>x &lt; 2</m> (values just to the left of <m>2</m>), we have <m>x-2 &lt; 0</m> while
    <m>x+2 &gt; 0</m>, so their product is negative:
    <m>(x-2)(x+2) &lt; 0</m>. Hence
    <m>\lvert x^2 - 4 \rvert = -\bigl(x^2 - 4\bigr) = -(x-2)(x+2)</m>.
  </p>

  <p>Compute the left–hand limit by simplifying (for <m>x \neq 2</m>):</p>
  <me>
    \lim_{x\to 2^-}\frac{|x^2-4|}{x-2}
    \;=\;\lim_{x\to 2^-}\frac{-(x-2)(x+2)}{x-2}
    \;=\;\lim_{x\to 2^-}\bigl(-(x+2)\bigr)
    \;=\;-4.
  </me>

  <p>
    For <m>x &gt; 2</m> (values just to the right of <m>2</m>), both factors are positive:
    <m>x-2 &gt; 0</m> and <m>x+2 &gt; 0</m>, so <m>(x-2)(x+2) &gt; 0</m>. Therefore
    <m>\lvert x^2 - 4 \rvert = x^2 - 4 = (x-2)(x+2)</m>.
  </p>

  <p>Compute the right–hand limit similarly (for <m>x \neq 2</m>):</p>
  <me>
    \lim_{x\to 2^+}\frac{|x^2-4|}{x-2}
    \;=\;\lim_{x\to 2^+}\frac{(x-2)(x+2)}{x-2}
    \;=\;\lim_{x\to 2^+}(x+2)
    \;=\;4.
  </me>

  <p>
    The one–sided limits are different (<m>-4</m> vs. <m>4</m>), so the two–sided limit
    <m>\displaystyle\lim_{x\to 2}\frac{|x^2-4|}{x-2}</m> does not exist.
  </p>

  <remark>
    <p>
      It is legitimate to cancel the factor <m>x-2</m> in the simplified expressions because
      we only consider <m>x</m> near (but not equal to) <m>2</m>. If helpful, you can also
      confirm this behavior numerically with a table of values approaching <m>2</m> from each
      side or by inspecting a graph.
    </p>
  </remark>
</solution>
    </example>
  </subsection>

  <subsection xml:id="ssec-squeeze">
    <title>Limits by Squeezing</title>

    <p>
      Some limits are difficult because the function oscillates or behaves erratically near the point. In such cases we use inequalities to bound the function above and below.
    </p>

    <example xml:id="ex-squeeze-1">
      <title>Squeezing Example</title>
      <statement>
        <p>
          Evaluate <m>\displaystyle \lim_{x\to 1} x + 4(x-1)^2\sin(\tfrac{1}{x-1})</m>.
        </p>
      </statement>
      <solution>
        <p>
          Since <m>-1 \leq \sin(\theta) \leq 1</m>,
        </p>
        <me>
          x - 4(x-1)^2 \leq x + 4(x-1)^2\sin\!\left(\tfrac{1}{x-1}\right) \leq x+4(x-1)^2.
        </me>
        <p>
          Both bounds approach 1 as <m>x\to 1</m>, so by the Squeeze Theorem the limit is 1.
        </p>
      </solution>
    </example>

    <theorem xml:id="thm-squeeze">
      <title>Squeeze Theorem</title>
      <statement>
        <p>
          Suppose <m>g(x) \leq f(x) \leq h(x)</m> for all <m>x</m> near <m>a</m> (except possibly <m>x=a</m>), and <m>\lim_{x\to a} g(x) = \lim_{x\to a} h(x) = L</m>. Then <m>\lim_{x\to a} f(x) = L</m>.
        </p>
      </statement>
    </theorem>
  </subsection>

  <subsection xml:id="ssec-oscillations">
    <title>Oscillating Functions</title>

    <p>
      Some functions oscillate so wildly near a point that the limit does not exist. For example, consider:
    </p>

    <example xml:id="ex-sin-pi-over-x">
      <title>Wild Oscillations</title>
      <statement>
        <p>
          Consider <m>\displaystyle \lim_{x\to 0} \sin\left(\frac{\pi}{x}\right)</m>.
        </p>
      </statement>
      <solution>
        <p>
          The function oscillates infinitely often as <m>x\to 0</m>, so it cannot be forced close to any single value. Thus the limit does not exist.
        </p>
      </solution>
    </example>

    <example xml:id="ex-xsin">
      <title>Oscillation with Decay</title>
      <statement>
        <p>
          Consider <m>\displaystyle \lim_{x\to 0} x\sin\left(\tfrac{\pi}{x}\right)</m>.
        </p>
      </statement>
      <solution>
        <p>
          Since <m>-1 \leq \sin(\tfrac{\pi}{x}) \leq 1</m>, we have <m>-|x| \leq x\sin(\tfrac{\pi}{x}) \leq |x|</m>. Both bounds approach 0, so by the Squeeze Theorem the limit equals 0.
        </p>
      </solution>
    </example>
  </subsection>
</section>
