<?xml version="1.0" encoding="UTF-8"?>

<section xml:id="sec-integral-usub" xmlns:xi="http://www.w3.org/2001/XInclude">
  <title>Substitution Rule for Integration</title>

  <objectives>
    <ul>
      <li>Recognize when an integrand has the form <m>f(g(x))g'(x)</m> and apply substitution.</li>
      <li>Use substitution to evaluate indefinite integrals and then check results by differentiation.</li>
      <li>Use substitution with updated limits to evaluate definite integrals.</li>
      <li>Use symmetry (odd functions) to evaluate certain definite integrals quickly.</li>
      <li>Model a real situation with an integral and interpret a substitution physically.</li>
    </ul>
  </objectives>

  <subsection xml:id="ssec-reverse-chain">
    <title>Reversing the Chain Rule</title>

    <p>
      By the Second Fundamental Theorem of Calculus, one efficient way to evaluate a definite integral
      <m>\displaystyle \int_a^b f(x)\,dx</m> is to find an antiderivative <m>F</m> and compute
      <m>F(b)-F(a)</m>. In this section we develop a powerful method for finding antiderivatives by
      reversing the Chain Rule:
      <m>\dfrac{d}{dx}\big(F(g(x))\big)=F'(g(x))g'(x)</m>.
    </p>

    <p>
      For example, consider the indefinite integral
      <m>\displaystyle \int x\cos(x^2)\,dx</m>.
      The inside function <m>g(x)=x^2</m> appears inside the cosine, and its derivative is <m>g'(x)=2x</m>.
      Since the integrand contains a factor <m>x</m>, we rewrite it to match the Chain Rule pattern:
    </p>

    <me>
      x\cos(x^2)
      \ =\
      \tfrac12\cos(x^2)\cdot (2x)
      \ =\
      \tfrac12\cos(x^2)\cdot (x^2)'.
    </me>

    <p>
      Now set <m>u=g(x)=x^2</m>. Then <m>du=g'(x)\,dx=2x\,dx</m>, so <m>\tfrac12\,du=x\,dx</m>, and the integral becomes
    </p>

    <me>
      \int x\cos(x^2)\,dx
      \ =\
      \tfrac12\int \cos(u)\,du
      \ =\
      \tfrac12\sin(u)+C
      \ =\
      \tfrac12\sin(x^2)+C.
    </me>

    <p>
      A quick check comes from the Chain Rule:
      if <m>F(x)=\tfrac12\sin(x^2)</m>, then
      <m>F'(x)=\tfrac12\cos(x^2)\cdot 2x=x\cos(x^2)</m>.
    </p>
  </subsection>

  <subsection xml:id="ssec-substitution-method">
    <title>Substitution Method</title>

    <p>
      Substitution is a structured way to reverse the Chain Rule. The goal is to rewrite the integrand so it looks like
      <m>f(g(x))g'(x)</m>.
    </p>

    <ol>
      <li>
        <p>
          Start with an integral <m>\int h(x)\,dx</m>. Look for an inside function <m>g(x)</m>
          so that <m>g'(x)</m> appears as a factor (possibly after multiplying and dividing by a constant):
        </p>
        <me>
          h(x)\ =\ f(g(x))\cdot g'(x).
        </me>
        <p>
          After factoring out <m>g'(x)</m>, rewrite the remaining part as a function of <m>u=g(x)</m>.
        </p>
      </li>

      <li>
        <p>
          Let <m>u=g(x)</m>, so <m>du=g'(x)\,dx</m>. Then rewrite the integral in <m>u</m>:
        </p>
        <me>
          \int h(x)\,dx
          \ =\
          \int f(g(x))g'(x)\,dx
          \ =\
          \int f(u)\,du.
        </me>
        <p>
          Compute <m>\int f(u)\,du</m> using basic antiderivatives and rules.
        </p>
      </li>

      <li>
        <p>
          Substitute back <m>u=g(x)</m> to express the final answer in terms of <m>x</m>:
        </p>
        <me>
          \int h(x)\,dx
          \ =\
          F(u)+C
          \ =\
          F(g(x))+C.
        </me>
      </li>
    </ol>
  </subsection>

  <subsection xml:id="ssec-substitution-examples">
    <title>Examples</title>

    <example xml:id="ex-sub-01">
      <statement>
        <p>
          Evaluate <m>\displaystyle \int (3x+4)\sqrt{3x+4}\,dx</m>.
        </p>
      </statement>
      <solution>
        <p>
          Let <m>u=3x+4</m>. Then <m>du=3\,dx</m>, so <m>dx=\tfrac13\,du</m>. Thus,
        </p>
        <me>
          \begin{array}{rcl}
          \displaystyle \int (3x+4)\sqrt{3x+4}\,dx
          &amp;=&amp;
          \displaystyle \int u\sqrt{u}\cdot \tfrac13\,du
          \\[0.8em]
          &amp;=&amp;
          \displaystyle \tfrac13\int u^{3/2}\,du
          \ =\
          \tfrac13\cdot \tfrac{2}{5}u^{5/2}+C
          \\[0.8em]
          &amp;=&amp;
          \displaystyle \tfrac{2}{15}(3x+4)^{5/2}+C.
          \end{array}
        </me>
      </solution>
    </example>

    <example xml:id="ex-sub-02">
      <statement>
        <p>
          Evaluate <m>\displaystyle \int x\sqrt{3x+4}\,dx</m>.
        </p>
      </statement>
      <solution>
        <p>
          Let <m>u=3x+4</m>, so <m>du=3\,dx</m> and <m>dx=\tfrac13\,du</m>.
          We also solve for <m>x</m>: <m>u=3x+4</m> gives <m>x=\tfrac13u-\tfrac43</m>.
        </p>

        <me>
          \begin{array}{rcl}
          \displaystyle \int x\sqrt{3x+4}\,dx
          &amp;=&amp;
          \displaystyle \int \left(\tfrac13u-\tfrac43\right)\sqrt{u}\cdot \tfrac13\,du
          \\[0.9em]
          &amp;=&amp;
          \displaystyle \int \left(\tfrac19u^{3/2}-\tfrac49u^{1/2}\right)\,du
          \\[0.9em]
          &amp;=&amp;
          \displaystyle \tfrac19\cdot \tfrac{2}{5}u^{5/2}-\tfrac49\cdot \tfrac{2}{3}u^{3/2}+C
          \\[0.9em]
          &amp;=&amp;
          \displaystyle \tfrac{2}{45}(3x+4)^{5/2}-\tfrac{8}{27}(3x+4)^{3/2}+C.
          \end{array}
        </me>
      </solution>
    </example>

    <example xml:id="ex-sub-03">
      <statement>
        <p>
          Evaluate <m>\displaystyle \int \frac{\sec^2(\sqrt{x})}{\sqrt{x}}\,dx</m>.
        </p>
      </statement>
      <solution>
        <p>
          Let <m>u=\sqrt{x}=x^{1/2}</m>. Then <m>du=\tfrac{1}{2}x^{-1/2}\,dx=\tfrac{1}{2\sqrt{x}}\,dx</m>.
          Rewrite to produce <m>du</m>:
        </p>

        <me>
          \begin{array}{rcl}
          \displaystyle \int \frac{\sec^2(\sqrt{x})}{\sqrt{x}}\,dx
          &amp;=&amp;
          \displaystyle \int 2\sec^2(\sqrt{x})\cdot \frac{1}{2\sqrt{x}}\,dx
          \\[0.9em]
          &amp;=&amp;
          \displaystyle \int 2\sec^2(u)\,du
          \ =\
          2\tan(u)+C
          \\[0.9em]
          &amp;=&amp;
          \displaystyle 2\tan(\sqrt{x})+C.
          \end{array}
        </me>
      </solution>
    </example>

    <example xml:id="ex-sub-04">
      <statement>
        <p>
          Evaluate <m>\displaystyle \int \frac{\sin(x)}{(1+\cos(x))^2}\,dx</m>.
        </p>
      </statement>
      <solution>
        <p>
          Let <m>u=1+\cos(x)</m>. Then <m>du=-\sin(x)\,dx</m>, so <m>\sin(x)\,dx=-du</m>.
        </p>

        <me>
          \begin{array}{rcl}
          \displaystyle \int \frac{\sin(x)}{(1+\cos(x))^2}\,dx
          &amp;=&amp;
          \displaystyle -\int \frac{1}{u^2}\,du
          \\[0.9em]
          &amp;=&amp;
          \displaystyle -\left(\frac{u^{-1}}{-1}\right)+C
          \ =\
          \frac{1}{u}+C
          \\[0.9em]
          &amp;=&amp;
          \displaystyle \frac{1}{1+\cos(x)}+C.
          \end{array}
        </me>
      </solution>
    </example>

    <example xml:id="ex-sub-05">
      <statement>
        <p>
          Evaluate <m>\displaystyle \int \sec^2(x)\tan(x)\,dx</m> in two ways, and explain why the answers agree.
        </p>
      </statement>
      <solution>
        <p>
          Method 1: Let <m>u=\tan(x)</m>. Then <m>du=\sec^2(x)\,dx</m>.
        </p>

        <me>
          \begin{array}{rcl}
          \displaystyle \int \sec^2(x)\tan(x)\,dx
          &amp;=&amp;
          \displaystyle \int u\,du
          \ =\
          \tfrac12 u^2 + C
          \ =\
          \tfrac12\tan^2(x)+C.
          \end{array}
        </me>

        <p>
          Method 2: Write the integrand as <m>\sec(x)\cdot (\tan(x)\sec(x))</m> and let <m>z=\sec(x)</m>.
          Then <m>dz=\tan(x)\sec(x)\,dx</m>.
        </p>

        <me>
          \begin{array}{rcl}
          \displaystyle \int \sec^2(x)\tan(x)\,dx
          &amp;=&amp;
          \displaystyle \int z\,dz
          \ =\
          \tfrac12 z^2 + C
          \ =\
          \tfrac12\sec^2(x)+C.
          \end{array}
        </me>

        <p>
          These differ by a constant because <m>\sec^2(x)=\tan^2(x)+1</m>.
          So <m>\tfrac12\sec^2(x)=\tfrac12\tan^2(x)+\tfrac12</m>, meaning the two antiderivative families are the same.
        </p>
      </solution>
    </example>
  </subsection>

  <subsection xml:id="ssec-substitution-definite">
    <title>Substitution for Definite Integrals</title>

    <p>
      Substitution can be used directly with definite integrals by changing the limits.
      If <m>u=g(x)</m>, then
    </p>

    <me>
      \int_a^b f(g(x))g'(x)\,dx \ =\ \int_{g(a)}^{g(b)} f(u)\,du.
    </me>

    <example xml:id="ex-sub-def-01">
      <statement>
        <p>
          Evaluate <m>\displaystyle \int_2^3 x(1+x^2)^5\,dx</m>.
        </p>
      </statement>
      <solution>
        <p>
          Let <m>u=1+x^2</m>, so <m>du=2x\,dx</m> and <m>x\,dx=\tfrac12\,du</m>.
          Update the limits: when <m>x=2</m>, <m>u=1+2^2=5</m>; when <m>x=3</m>, <m>u=1+3^2=10</m>.
        </p>

        <me>
          \begin{array}{rcl}
          \displaystyle \int_2^3 x(1+x^2)^5\,dx
          &amp;=&amp;
          \displaystyle \int_2^3 \tfrac12 (1+x^2)^5\cdot 2x\,dx
          \\[0.9em]
          &amp;=&amp;
          \displaystyle \int_{5}^{10} \tfrac12 u^5\,du
          \ =\
          \left.\tfrac{1}{12}u^6\right|_{u=5}^{u=10}
          \\[0.9em]
          &amp;=&amp;
          \displaystyle \tfrac{1}{12}\left(10^6-5^6\right).
          \end{array}
        </me>
      </solution>
    </example>
  </subsection>

  <subsection xml:id="ssec-integral-symmetry">
    <title>Integral Symmetry for Odd Functions</title>

    <theorem xml:id="thm-integral-symmetry-odd">
      <title>Integral Symmetry Theorem</title>
      <statement>
        <p>
          If <m>f</m> is odd, meaning <m>f(-x)=-f(x)</m>, then for any <m>a&gt;0</m>,
        </p>
        <me>
          \int_{-a}^{a} f(x)\,dx \ =\ 0.
        </me>
      </statement>
    </theorem>

    <proof>
      <p>
        By the splitting rule,
      </p>
      <me>
        \int_{-a}^{a} f(x)\,dx \ =\ \int_{-a}^{0} f(x)\,dx + \int_{0}^{a} f(x)\,dx.
      </me>
      <p>
        In the first integral, substitute <m>u=-x</m>, so <m>du=-dx</m>.
        When <m>x=-a</m>, <m>u=a</m>; when <m>x=0</m>, <m>u=0</m>. Then:
      </p>
      <me>
        \begin{array}{rcl}
        \displaystyle \int_{-a}^{0} f(x)\,dx
        &amp;=&amp;
        \displaystyle \int_{a}^{0} f(-u)\,(-du)
        \ =\
        \int_{a}^{0} (-f(u))\,(-du)
        \\[0.9em]
        &amp;=&amp;
        \displaystyle \int_{a}^{0} f(u)\,du
        \ =\
        -\int_{0}^{a} f(u)\,du.
        \end{array}
      </me>
      <p>
        Therefore <m>\int_{-a}^{0} f(x)\,dx + \int_{0}^{a} f(x)\,dx=0</m>.
      </p>
    </proof>

    <example xml:id="ex-odd-symmetry-01">
      <statement>
        <p>
          Evaluate <m>\displaystyle \int_{-\pi}^{\pi} x\cos(x)\,dx</m>.
        </p>
      </statement>
      <solution>
        <p>
          The integrand <m>f(x)=x\cos(x)</m> is odd because
          <m>f(-x)=(-x)\cos(-x)=(-x)\cos(x)=-f(x)</m>. By the symmetry theorem,
        </p>
        <me>
          \int_{-\pi}^{\pi} x\cos(x)\,dx \ =\ 0.
        </me>
      </solution>
    </example>

    <figure xml:id="fig-xcosx">
      <caption>
        <p>
          The graph of <m>y=x\cos(x)</m> is rotationally symmetric about the origin, so the signed areas on <m>[-\pi,0]</m> and <m>[0,\pi]</m> cancel.
        </p>
      </caption>
      <image source="4-5-XCosX.png" width="60%"/>
    </figure>
  </subsection>

  <subsection xml:id="ssec-heart-flow">
    <title>Application: Heart Flow Rate</title>

    <p>
      In a medical test, a known amount of dye is injected into a vein flowing toward the heart.
      Let <m>c(t)</m> be the measured dye concentration in arterial blood (mg per liter) at time <m>t</m> minutes.
      If the (unknown) blood flow rate is constant at <m>r</m> liters per minute, then the total blood volume that has passed is <m>\ell=rt</m>.
      Let <m>C(\ell)</m> be the dye concentration after <m>\ell</m> liters have passed, so <m>C(rt)=c(t)</m>.
    </p>

    <p>
      The total amount of dye <m>D</m> (in mg) can be computed by integrating concentration with respect to volume:
    </p>

    <me>
      D \ =\ \int_0^{\infty} C(\ell)\,d\ell.
    </me>

    <p>
      Substitute <m>\ell=rt</m>, so <m>d\ell=r\,dt</m> and <m>C(\ell)=C(rt)=c(t)</m>. Then
    </p>

    <me>
      \begin{array}{rcl}
      \displaystyle D
      &amp;=&amp;
      \displaystyle \int_0^{\infty} C(\ell)\,d\ell
      \ =\
      \int_0^{\infty} C(rt)\,r\,dt
      \\[0.9em]
      &amp;=&amp;
      \displaystyle r\int_0^{\infty} c(t)\,dt.
      \end{array}
    </me>

    <p>
      Solving for the flow rate gives
    </p>

    <me>
      r \ =\ \frac{D}{\displaystyle \int_0^{\infty} c(t)\,dt}.
    </me>

    <p>
      In practice, once the dye has passed through the system, <m>c(t)</m> becomes (essentially) zero, so the improper integral can be replaced by a finite upper limit chosen from the data.
      The remaining integral can be approximated numerically (for example, by a Riemann sum or a spreadsheet).
    </p>
  </subsection>

<subsection xml:id="additional-worked-problems-integral-usub">
  <title>Additional Worked-Out Examples</title>

  <p>
    To keep this section at a reasonable length, we include only a few representative examples directly in the text.
    If you find yourself stuck on a homework problem, or if you are studying before a quiz or exam, additional
    fully worked-out examples are available via: 
    <alert>
      <xref ref="subsec-integral-usub">
        Additional Worked-Out Problems for Substitution Rule for Integration
      </xref>
    </alert>
  </p>

</subsection>


  <exercises xml:id="exercises-substitution">
    <title>Practice / Study Problems</title>

    <exercisegroup>
      <title>Indefinite Integrals by Substitution</title>

      <exercise xml:id="prob-sub-01">
        <statement>
          <p>Compute <m>\displaystyle \int 6x(1+x^2)^4\,dx</m>.</p>
        </statement>
      </exercise>

      <exercise xml:id="prob-sub-02">
        <statement>
          <p>Compute <m>\displaystyle \int \frac{e^{3x}}{1+e^{3x}}\,dx</m>.</p>
        </statement>
      </exercise>

      <exercise xml:id="prob-sub-03">
        <statement>
          <p>Compute <m>\displaystyle \int \sin(5x)\,dx</m> and check by differentiating.</p>
        </statement>
      </exercise>
    </exercisegroup>

    <exercisegroup>
      <title>Definite Integrals and Symmetry</title>

      <exercise xml:id="prob-sub-def-01">
        <statement>
          <p>Evaluate <m>\displaystyle \int_0^1 2x\sqrt{1+x^2}\,dx</m> using substitution with updated limits.</p>
        </statement>
      </exercise>

      <exercise xml:id="prob-odd-01">
        <statement>
          <p>Without finding an antiderivative, evaluate <m>\displaystyle \int_{-4}^{4} (x^3-2x)\,dx</m>.</p>
        </statement>
      </exercise>
    </exercisegroup>
  </exercises>

</section>