<?xml version="1.0" encoding="UTF-8"?>

<section xml:id="sec-derivative-intro" xmlns:xi="http://www.w3.org/2001/XInclude">
  <title>Introduction and Motivation for Derivatives</title>

<objectives>
  <ul>
    <li>
      Compute the average rate of change of a function on an interval and interpret it as the slope of a secant line.
    </li>
    <li>
      Describe instantaneous velocity as the limit of average velocities over shrinking time intervals.
    </li>
    <li>
      Interpret instantaneous rate of change geometrically as the slope of a tangent line.
    </li>
    <li>
      Use tables, graphs, and nearby average rates of change to estimate an instantaneous rate of change.
    </li>
  </ul>
</objectives>

  <p>
    Derivatives begin with a simple question: how fast is something changing <em>right now</em>?
    You already know how to compute an <em>average</em> rate of change over a time interval.
    The derivative is what happens when we shrink that interval smaller and smaller and study the
    limiting behavior of these average rates.
  </p>

  <p>
    Throughout this section, the same expression will appear in multiple contexts:
    average velocity, slopes of secant lines, and instantaneous rate of change.
    This expression is called the <em>difference quotient</em>.
  </p>

<subsection xml:id="instantaneous-velocity">
  <title>Average and Instantaneous Velocity</title>

  <p>
    Suppose a particle moves along a line so that at time <m>t</m> it is at position <m>f(t)</m>.
    We begin by defining the average velocity over a time interval.
  </p>

  <definition xml:id="def-average-velocity">
    <statement>
      <p>
        Let <m>f(t)</m> denote the position of an object at time <m>t</m>.
        The <term>average velocity</term> of the object on the time interval
        <m>[a,b]</m> is
      </p>
      <me>
        \displaystyle v_{\mathrm{avg}}=\frac{f(b)-f(a)}{b-a}.
      </me>
    </statement>
  </definition>

  <remark xml:id="rem-avg-velocity-interpretation">
    <p>
      The average velocity represents the total change in position divided by the total
      change in time. Geometrically, it is the slope of the secant line connecting
      <m>(a,f(a))</m> and <m>(b,f(b))</m> on the graph of <m>y=f(t)</m>.
    </p>
  </remark>

  <p>
    Instantaneous velocity cannot be measured over a single moment in time.
    Instead, it is defined as a limit of average velocities over shrinking time intervals.
  </p>

  <definition xml:id="def-instantaneous-velocity">
    <statement>
      <p>
        Let <m>f(t)</m> denote the position of an object at time <m>t</m>.
        The <term>instantaneous velocity</term> at time <m>t=a</m> is
      </p>
      <me>
        \displaystyle v=\lim_{h\to 0}\frac{f(a+h)-f(a)}{h},
      </me>
      <p>
        provided this limit exists. More generally, if <m>f(t)</m> represents a quantity other than position,
      this same limit represents the <term>instantaneous rate of change</term>
      of that quantity with respect to time at <m>t = a</m>.
      </p>
    </statement>
  </definition>

  <remark xml:id="rem-velocity-speed">
    <p>
      Velocity may be positive or negative depending on direction of motion.
      The <em>speed</em> of an object is the absolute value of its velocity.
    </p>
  </remark>


<example xml:id="ex-falling-stone">
  <introduction>
    <p>
      A stone dropped from a bridge has position (in feet below the bridge)
      approximately <m>f(t)=16t^2</m> after <m>t</m> seconds.
    </p>
  </introduction>

  <task>
    <statement>
      <p>
        Compute the average velocity on <m>[3,4]</m> using <xref ref="def-average-velocity"/>.
      </p>
    </statement>
    <solution>
      <p>
        Using <xref ref="def-average-velocity"/> with <m>a=3</m> and <m>b=4</m>,
      </p>
      <me>
\displaystyle
\begin{array}{rcl}
v_{\mathrm{avg}}
&amp;=&amp; \displaystyle \frac{f(4)-f(3)}{4-3}
\\[0.8em]
&amp;=&amp; \displaystyle \frac{16(4^2)-16(3^2)}{1}
\\[0.8em]
&amp;=&amp; \displaystyle 16(16-9)
\\[0.8em]
&amp;=&amp; \displaystyle 112.
\end{array}
      </me>
      <p>
        So the average velocity on <m>[3,4]</m> is <m>112</m> ft/sec.
      </p>
    </solution>
  </task>

  <task>
    <statement>
      <p>
        Use the table of velocities below to estimate the instantaneous velocity at <m>t=3</m>.
      </p>

      <me>
\displaystyle
\begin{array}{c|ccccc}
h
&amp; 1
&amp; 0.1
&amp; 0.01
&amp; 0.001
&amp; 0.0001
\\ \hline
v_{\mathrm{avg}}
&amp; 112
&amp; 97.6
&amp; 96.16
&amp; 96.016
&amp; 96.0016
\end{array}
      </me>
    </statement>
    <solution>
      <p>
        As <m>h</m> gets smaller, the average velocities get closer to <m>96</m>.
        So a reasonable estimate for the instantaneous velocity at <m>t=3</m> is
        <m>96</m> ft/sec.
      </p>
    </solution>
  </task>

  <task>
    <statement>
      <p>
        Compute the instantaneous velocity at <m>t=3</m> using <xref ref="def-instantaneous-velocity"/>.
      </p>
    </statement>
    <solution>
      <p>
        By <xref ref="def-instantaneous-velocity"/>, the instantaneous velocity at <m>t=3</m> is
      </p>

      <me>
v = \displaystyle\lim_{h\to 0}\frac{f(3+h)-f(3)}{h}.
      </me>

      <p>
        Since <m>f(t)=16t^2</m>, we compute
      </p>

      <me>
\displaystyle
\begin{array}{rcl}
v
&amp;=&amp; \displaystyle \lim_{h\to 0}\frac{16(3+h)^2-16(3^2)}{h}
\\[0.9em]
&amp;=&amp; \displaystyle \lim_{h\to 0}16\cdot\frac{(3+h)^2-9}{h}
\\[0.9em]
&amp;=&amp; \displaystyle \lim_{h\to 0}16\cdot\frac{(9+6h+h^2)-9}{h}
\\[0.9em]
&amp;=&amp; \displaystyle \lim_{h\to 0}16\cdot\frac{6h+h^2}{h}
\\[0.9em]
&amp;=&amp; \displaystyle \lim_{h\to 0}16(6+h)
\\[0.9em]
&amp;=&amp; \displaystyle \lim_{h\to 0}96+16h
\end{array}
      </me>

      <p>
        As we take <m>h</m> smaller and smaller, the error term <m>16h</m> approaches zero, and
the average velocity approaches the limiting value <m>96</m>, which by definition is
the instantaneous velocity.
        Therefore, the instantaneous velocity at <m>t=3</m> is <m>96</m> ft/sec.
      </p>
    </solution>
  </task>
</example>

  </subsection>

<subsection xml:id="secant-and-tangent">
  <title>Slopes of Secant Lines and Slopes of Tangent Lines</title>

  <p>
    We have described velocity on several conceptual levels.
    It can be understood as a <em>physical</em> quantity describing motion,
    a <em>numerical</em> approximation obtained from average rates of change,
    and an <em>algebraic</em> computation using limits.
    Velocity also has a <em>geometric</em> interpretation in terms of the graph
    <m>y=f(t)</m>, where it corresponds to the slope of the graph at a given time.
  </p>

  <p>
    A <term>secant line</term> is a line that passes through two distinct points on the graph.
    It cuts across the curve and represents how the function changes between two different
    input values.
    When these two points are far apart, the secant line gives a coarse description of the
    function’s behavior over an interval.
  </p>

  <sidebyside width="80%">
    <figure xml:id="secant-line">
      <caption>
        A secant line connecting the points <m>(1,f(1))</m> and <m>(7,f(7))</m>,
        representing the average rate of change of <m>f</m> on the interval <m>[1,7]</m>.
      </caption>
      <image source="images/secant01.png" width="100%"/>
    </figure>
  </sidebyside>

  <definition xml:id="def-secant-slope">
    <statement>
      <p>
        Let <m>f</m> be a function and let <m>a \neq b</m>.
        The <term>slope of the secant line</term> to <m>f</m> between <m>x=a</m> and <m>x=b</m> is
      </p>
      <me>
        \displaystyle m_{\mathrm{sec}}=\frac{f(b)-f(a)}{b-a}.
      </me>
    </statement>
  </definition>

  <remark xml:id="rem-secant-interpretation">
    <p>
      The slope of the secant line is the slope of the line through the points
      <m>(a,f(a))</m> and <m>(b,f(b))</m>.
      Algebraically, it is the same formula used for the average rate of change.
    </p>
  </remark>

  <p>
    A <term>tangent line</term>, on the other hand, touches the graph at a single point and
    matches the direction of the curve at that point.
    The tangent line represents the best linear approximation to the function near a specific point.
  </p>

  <sidebyside width="80%">
    <figure xml:id="tangent-line">
      <caption>
        A tangent line through the point <m>(1,f(1))</m>,
        representing the instantaneous rate of change of <m>f</m> at <m>x=1</m>.
      </caption>
      <image source="images/tangent01.png" width="100%"/>
    </figure>
  </sidebyside>

  <p>
    As the second point used to define a secant line moves closer and closer to the first,
    the secant line approaches the tangent line.
    This idea leads directly to the following definitions.
  </p>

  <url href="https://www.desmos.com/calculator/sw9jjcgdeh">
        <sidebyside width="80%">
                <figure>
                          <caption>
                                      As two points on the curve move closer together, the secant line
                                                determined by those points approaches the tangent line at a single point.
                          </caption>
                                  <image width="100%" source="images/tangentSecant.gif">
                                              <shortdescription>
                                                            Animated graph of a smooth curve with two points marked on it. A secant line passes
                                                                        through the two points. As the points move closer together along the curve,
                                                                                    the secant line rotates and converges to the tangent line at that point, illustrating how the tangent
                                                                                                line arises as a limit of secant lines.
                                              </shortdescription>
                                            </image>
                                          </figure>
                                        </sidebyside>
                                      </url>

  <definition xml:id="def-tangent-slope">
    <statement>
      <p>
        Let <m>f</m> be a function and let <m>a</m> be a point in its domain.
        The <term>slope of the tangent line</term> to <m>f</m> at <m>x = a</m> is
      </p>
      <me>
        \displaystyle m = \lim_{x \to a} \frac{f(x) - f(a)}{x - a},
      </me>
      <p>
        provided this limit exists.
        Equivalently, the slope of the tangent line can be written as
      </p>
      <me>
        \displaystyle m = \lim_{h \to 0} \frac{f(a+h) - f(a)}{h},
      </me>
      <p>
        provided this limit exists.
      </p>
    </statement>
  </definition>

  <remark>
    <p>
      The limit as <m>h \to 0</m> is the more common definition in practice,
      because it is often algebraically convenient to evaluate limits at
      <m>h = 0</m> after simplifying the expression.
    </p>
  </remark>

  <remark xml:id="rem-tangent-connection">
    <p>
      The slope of the tangent line gives the slope of the line that best approximates the graph of
      <m>y=f(x)</m> near <m>x=a</m>.
      This is the same limit used to define instantaneous velocity, which explains why
      this limit describes both slopes of curves and rates of change.
    </p>
  </remark>

  <p>At this stage, tables and graphs allow us to estimate instantaneous rates of change. Exact values will come from limits.
  </p>


  <example xml:id="ex-temperature-average-rates">
    <title>A Trigonometric Model and Estimating Rates</title>
    <statement>
      <p>
        We model average daily temperature through
        the year by the sinusoidal function:
      </p>
      <me>
        \displaystyle
        T(x)=55-40\cos\!\left(\frac{2\pi}{365}x\right),
        \quad\text{degrees F on day } x.
      </me>
      <p>
        Using this model we found that
      </p>
      <me>
\begin{array}{c|c|c}
\text{Day} &amp; x &amp; T(x) \\ \hline
\text{Mar 31} &amp; 90  &amp; 54.1 \\
\text{Apr 10} &amp; 100 &amp; 61.0 \\
\text{Apr 20} &amp; 110 &amp; 67.7
\end{array}
      </me>
      <p>
        Using this table, estimate how quickly the weather is warming at <m>x=100</m>
        (Apr 10), in degrees per day.
      </p>
    </statement>

    <solution>
      <p>
        To estimate how quickly the temperature is changing at <m>x = 100</m>,
        we approximate the instantaneous rate of change using average rates of change
        from nearby data values in the table.
      </p>

      <p>
        First, compute the average rate of change from <m>x = 90</m> to <m>x = 100</m>.
      </p>

      <me>
\begin{array}{rcl}
\dfrac{T(100) - T(90)}{100 - 90}
&amp; = &amp;
\dfrac{61.0 - 54.1}{10} \\[0.6em]
&amp; = &amp;
\dfrac{6.9}{10} \\[0.6em]
&amp; = &amp;
0.69
\end{array}
      </me>

      <p>
        Next, compute the average rate of change from <m>x = 100</m> to <m>x = 110</m>.
      </p>

      <me>
\begin{array}{rcl}
\dfrac{T(110) - T(100)}{110 - 100}
&amp; = &amp;
\dfrac{67.7 - 61.0}{10} \\[0.6em]
&amp; = &amp;
\dfrac{6.7}{10} \\[0.6em]
&amp; = &amp;
0.67
\end{array}
      </me>

      <p>
        These two values represent average rates of change on either side of
        <m>x = 100</m>.
        Since they are close in value, we use their average to estimate
        the instantaneous rate of change at <m>x = 100</m>.
      </p>

      <me>
\begin{array}{rcl}
\text{Estimated rate at } x = 100
&amp; \approx &amp;
\dfrac{0.69 + 0.67}{2} \\[0.6em]
&amp; = &amp;
0.68
\end{array}
      </me>

      <p>
        Therefore, the temperature is increasing at approximately
        <m>0.68</m> degrees Fahrenheit per day on April 10.
      </p>
    </solution>
  </example>

  <p>
    In the next sections, we will turn these ideas into a precise definition
    and develop tools for computing instantaneous rates of change efficiently.
  </p>
</subsection>

<subsection xml:id="additional-worked-problems-derivIntro">
  <title>Additional Worked-Out Examples</title>

  <p>
    To keep this section at a reasonable length, we include only a few representative examples directly in the text.
    If you find yourself stuck on a homework problem, or if you are studying before a quiz or exam, additional
    fully worked-out examples are available via: 
    <alert>
      <xref ref="subsec-deriv-intro">
        Additional Examples for Introduction and Motivation for Derivatives 
      </xref>
    </alert>
  </p>

</subsection>






<exercises xml:id="exercises-derivative-intro-tf">
  <title>Practice / Study Problems</title>

  <exercisegroup>
    <title>Some True/False Problems</title>
    <introduction>
      <p>
        Determine whether each statement is true or false and explain your reasoning
      </p>
    </introduction>

    <!-- Average rate of change computations -->

 <exercise xml:id="tf-deriv-intro-01">
  <statement>
    <p>
      If <m>f(x)=x^2</m>, then the average rate of change of <m>f</m> on <m>[2,5]</m> is <m>7</m>.
    </p>
  </statement>
  <solution>
    <p>
      <em>True.</em> The average rate of change on <m>[2,5]</m> is
    </p>
    <me>
      \displaystyle \frac{f(5)-f(2)}{5-2}
      =
      \frac{25-4}{3}
      =
      7.
    </me>
  </solution>
</exercise>

<exercise xml:id="tf-deriv-intro-02">
  <statement>
    <p>
      The average rate of change of <m>f(x)=3x-1</m> on any interval is <m>3</m>.
    </p>
  </statement>
  <solution>
    <p>
      <em>True.</em> On <m>[a,b]</m>,
    </p>
    <me>
      \displaystyle \frac{f(b)-f(a)}{b-a}
      =
      \frac{(3b-1)-(3a-1)}{b-a}
      =
      \frac{3(b-a)}{b-a}
      =
      3.
    </me>
  </solution>
</exercise>


<exercise xml:id="tf-deriv-intro-04">
  <statement>
    <p>
      If <m>f(x)=x^2</m>, then the average rate of change on <m>[a,a+h]</m> is <m>2a+h</m>.
    </p>
  </statement>
  <solution>
    <p>
      <em>True</em> (for <m>h\neq 0</m>). Compute
    </p>
    <me>
      \displaystyle \frac{f(a+h)-f(a)}{(a+h)-a}
      =
      \frac{(a+h)^2-a^2}{h}.
    </me>
    <p>
      Expand and simplify:
    </p>
    <me>
      \displaystyle \frac{(a^2+2ah+h^2)-a^2}{h}
      =
      \frac{2ah+h^2}{h}
      =
      2a+h.
    </me>
  </solution>
</exercise>

<exercise xml:id="tf-deriv-intro-05">
  <statement>
    <p>
      For <m>f(x)=x^2</m>, the slope of the tangent line to the graph of <m>y=f(x)</m>
      at <m>x=3</m> is <m>6</m>.
    </p>
  </statement>
  <solution>
    <p>
      <em>True.</em> By the definition of the slope of the tangent line,
    </p>
    <me>
      \displaystyle m=\lim_{h\to 0}\frac{f(3+h)-f(3)}{h}
      =
      \lim_{h\to 0}\frac{(3+h)^2-9}{h}.
    </me>
    <p>
      Expand and simplify:
    </p>
    <me>
      \displaystyle \lim_{h\to 0}\frac{9+6h+h^2-9}{h}
      =
      \lim_{h\to 0}\frac{6h+h^2}{h}
      =
      \lim_{h\to 0}(6+h)
      =
      6.
    </me>
  </solution>
</exercise>

<exercise xml:id="tf-deriv-intro-07">
  <statement>
    <p>
      If <m>f(x)=5</m>, then the slope of the tangent line to the graph of <m>y=f(x)</m>
      is <m>0</m> at every point <m>x=a</m>.
    </p>
  </statement>
  <solution>
    <p>
      <em>True.</em> Using the definition,
    </p>
    <me>
      \displaystyle m=\lim_{h\to 0}\frac{f(a+h)-f(a)}{h}
      =
      \lim_{h\to 0}\frac{5-5}{h}
      =
      \lim_{h\to 0} 0
      =
      0.
    </me>
    <p>
      This matches the geometric fact that the graph <m>y=5</m> is a horizontal line.
    </p>
  </solution>
</exercise>

<exercise xml:id="tf-deriv-intro-08">
  <statement>
    <p>
      If the position of an object at time <m>t</m> is given by <m>f(t)=t^3</m>,
      then the instantaneous velocity of the object at <m>t=2</m> is <m>12</m>.
    </p>
  </statement>
  <solution>
    <p>
      <em>True.</em> Instantaneous velocity at <m>t=2</m> is defined by
    </p>
    <me>
      \displaystyle v=\lim_{h\to 0}\frac{f(2+h)-f(2)}{h}
      =
      \lim_{h\to 0}\frac{(2+h)^3-2^3}{h}.
    </me>
    <p>
      Expand <m>(2+h)^3=8+12h+6h^2+h^3</m>. Then
    </p>
    <me>
      \displaystyle v
      =
      \lim_{h\to 0}\frac{(8+12h+6h^2+h^3)-8}{h}
      =
      \lim_{h\to 0}\frac{12h+6h^2+h^3}{h}.
    </me>
    <p>
      Simplify and evaluate:
    </p>
    <me>
      \displaystyle v
      =
      \lim_{h\to 0}(12+6h+h^2)
      =
      12.
    </me>
  </solution>
</exercise>

<exercise xml:id="tf-deriv-intro-09">
  <statement>
    <p>
      If <m>f(x)=\sqrt{x}</m>, then
      <m>\displaystyle\lim_{h\to 0}\frac{f(4+h)-f(4)}{h}=\frac{1}{2}</m>.
    </p>
  </statement>
  <solution>
    <p>
      <em>False.</em> Compute
    </p>
    <me>
      \displaystyle \lim_{h\to 0}\frac{\sqrt{4+h}-2}{h}.
    </me>
    <p>
      Multiply numerator and denominator by the conjugate <m>\sqrt{4+h}+2</m>:
    </p>
    <me>
      \displaystyle \lim_{h\to 0}\frac{\sqrt{4+h}-2}{h}\cdot\frac{\sqrt{4+h}+2}{\sqrt{4+h}+2}
      =
      \lim_{h\to 0}\frac{(4+h)-4}{h(\sqrt{4+h}+2)}.
    </me>
    <p>
      Simplify and evaluate:
    </p>
    <me>
      \displaystyle \lim_{h\to 0}\frac{h}{h(\sqrt{4+h}+2)}
      =
      \lim_{h\to 0}\frac{1}{\sqrt{4+h}+2}
      =
      \frac{1}{4} \neq \frac12.
    </me>
  </solution>
</exercise>

<exercise xml:id="tf-deriv-intro-10">
  <statement>
    <p>
      If average rates of change computed using <m>h=0.1</m> and <m>h=0.01</m>
      are very close in value, then that common value is a reasonable estimate
      of the instantaneous rate of change.
    </p>
  </statement>
  <solution>
    <p>
      <em>True.</em> The instantaneous rate of change is defined as a limit of average rates of change as
      <m>h\to 0</m>.
      If two average rates from small values of <m>h</m> are close, that suggests the values are stabilizing,
      and the shared value is a reasonable estimate of the limiting value.
    </p>
  </solution>
</exercise>

<exercise xml:id="tf-deriv-intro-11">
  <statement>
    <p>
      Estimates of instantaneous velocity obtained from tables are exact values.
    </p>
  </statement>
  <solution>
    <p>
      <em>False.</em> A table provides approximate values of average velocity for small but nonzero time steps.
      Unless we compute the actual limit, the value from the table is only an estimate of the instantaneous velocity.
    </p>
  </solution>
</exercise>

<exercise xml:id="tf-deriv-intro-14">
  <statement>
    <p>
      A negative instantaneous velocity means the object’s position is decreasing
      at that moment.
    </p>
  </statement>
  <solution>
    <p>
      <em>True.</em> Instantaneous velocity is the instantaneous rate of change of position.
      If <m>v&lt;0</m> at a moment, then position is decreasing at that moment, meaning the object is moving in the negative direction.
    </p>
  </solution>
</exercise>

<exercise xml:id="tf-deriv-intro-15">
  <statement>
    <p>
      The slope of the tangent line at <m>x=a</m> is the limit of slopes of secant lines
      through <m>(a,f(a))</m> and <m>(a+h,f(a+h))</m> as <m>h\to 0</m>.
    </p>
  </statement>
  <solution>
    <p>
      <em>True.</em> The slope of the secant line through <m>(a,f(a))</m> and <m>(a+h,f(a+h))</m> is
      <m>\dfrac{f(a+h)-f(a)}{h}</m>.
      The slope of the tangent line is defined as the limit of these secant slopes as <m>h\to 0</m>.
    </p>
  </solution>
</exercise>

<exercise xml:id="tf-deriv-intro-16">
  <statement>
    <p>
      If all nearby secant line slopes are increasing as <m>h\to 0</m>,
      then the slope of the tangent line must be infinite.
    </p>
  </statement>
  <solution>
    <p>
      <em>False.</em> Secant slopes can increase as the second point approaches <m>a</m> and still approach a finite limit.
      For example, for <m>f(x)=x^2</m> at <m>a=0</m>, the secant slopes
      <m>\dfrac{f(h)-f(0)}{h}=\dfrac{h^2}{h}=h</m> increase as <m>h</m> increases, but as <m>h\to 0</m> the slopes approach <m>0</m>, which is finite.
    </p>
  </solution>
</exercise>

<exercise xml:id="tf-deriv-intro-18">
  <statement>
    <p>
      If <m>\displaystyle\lim_{h\to 0}\frac{f(a+h)-f(a)}{h}=0</m>,
      then <m>f</m> has a horizontal tangent line at <m>x=a</m>.
    </p>
  </statement>
  <solution>
    <p>
      <em>True.</em> The expression
      <m>\displaystyle\lim_{h\to 0}\frac{f(a+h)-f(a)}{h}</m>
      is the slope of the tangent line at <m>x=a</m>, provided it exists.
      If that slope equals <m>0</m>, then the tangent line has slope <m>0</m>, which means it is horizontal.
    </p>
  </solution>
</exercise>

<exercise xml:id="tf-deriv-intro-19">
  <statement>
    <p>
      Two different functions can have the same average rate of change on an interval
      but different instantaneous rates of change at a point in that interval.
    </p>
  </statement>
  <solution>
    <p>
      <em>True.</em> The average rate of change depends only on endpoint values, but instantaneous rate of change depends on local behavior.
      For example, on <m>[0,2]</m> let
      <m>f(x)=x</m> and <m>g(x)=x+\sin(\pi x)</m>.
      Then <m>f(0)=g(0)=0</m> and <m>f(2)=g(2)=2</m>, so both have the same average rate of change:
      <m>\dfrac{2-0}{2-0}=1</m>.
      But at <m>x=1</m>, their instantaneous rates differ:
      <m>f</m> has slope <m>1</m>, while <m>g</m> has a different slope because of the sinusoidal term.
    </p>
  </solution>
</exercise>



</exercisegroup>
</exercises> 


</section>
