<?xml version="1.0" encoding="UTF-8"?>

<section xml:id="sec-derivative-trig" xmlns:xi="http://www.w3.org/2001/XInclude">
  <title>Trigonometric Derivatives</title>

  <objectives>
    <ul>
      <li>Use geometric and graphical reasoning to understand why <m>\sin'(x)=\cos(x)</m> and <m>\cos'(x)=-\sin(x)</m>.</li>
      <li>Use these results with the product and quotient rules to differentiate the remaining trigonometric functions.</li>
      <li>Evaluate basic trigonometric limits by rewriting them in terms of <m>\displaystyle \frac{\sin(u)}{u}</m>.</li>
      <li>Remember that standard trigonometric derivative formulas assume angles are measured in radians.</li>
    </ul>
  </objectives>

  <subsection xml:id="derivative-of-sine-and-cosine">
    <title>Derivative of Sine and Cosine</title>

    <p>
      Sine and cosine are fundamental for describing periodic motion. One way to predict their derivatives is to look at graphs.
      If we estimate the slope of the graph <m>y=\sin(x)</m> at many points, we can sketch its derivative function.
      The slopes appear to match the graph of <m>\cos(x)</m>.
    </p>


  <url href="https://www.desmos.com/calculator/czwxvlzlg0">
      <figure>
<caption>
The derivative of <m>\sin(x)</m> visualized: the slope of the tangent line to <m>y=\sin(x)</m> at each point matches the value of <m>\cos(x)</m>.
</caption>
        <image width="100%" source="images/DerivSineVsCosine.gif">
      <shortdescription>
    An animated graph showing a sine curve and a cosine curve. As a point moves along the sine curve, a tangent line is drawn. 
    The steepness of the tangent line changes and matches the height of the cosine curve at the same horizontal position.
      </shortdescription>
        </image>
      </figure>
  </url>


    <theorem xml:id="thm-derivative-sin-cos">
      <statement>
        <p>
          For all real <m>x</m> (measured in radians),
          <me>(\sin(x))'=\cos(x) \quad \text{ and } \quad (\cos(x))'=-\sin(x)</me>
        </p>
      </statement>

  <proof>
    <p>
      A full proof of these derivative formulas begins with the limit definition of the derivative applied to the sine and cosine functions.
      Using trigonometric identities, this reduces the problem to understanding the behavior of certain key limits involving sine and cosine near zero.
    </p>

    <p>
      The first half of this argument is presented clearly in the video
      <url href="https://youtu.be/j1n6AMuMQso?si=rOoM1UxhMYV6VoXW">Derivatives of Sine and Cosine from First Principles</url>.
      As you will see, completing the proof requires evaluating limits such as the limit of sine of x over x as x approaches zero, 
      which we will develop later in this section.
    </p>
  </proof>
    </theorem>

<p>
  For the time being, we will take this result as given and focus on how to use 
  it to find the derivative formulas for the other standard trigonometric functions.
</p>

</subsection>

  <subsection xml:id="general-trig-derivatives">
    <title>General Trigonometric Derivatives</title>

<p>
  Now that we know the derivatives of sine and cosine, we can quickly find the derivatives of the 
  remaining trigonometric functions by applying our basic differentiation rules, such as the Quotient Rule.
</p>

<theorem xml:id="thm-derivative-tan">
  <statement>
    <p>
      For all real <m>x</m> such that <m>\tan(x)</m> is defined,
      <me>
        (\tan(x))' = \sec^2(x).
      </me>
    </p>
  </statement>
  <proof>
    <p>
      Recall that <m>\tan(x)=\dfrac{\sin(x)}{\cos(x)}</m>. Since <m>\cos(x)\neq 0</m> wherever <m>\tan(x)</m> is defined, we may apply the Quotient Rule.
    </p>

    <me>
      \begin{array}{rcl}
        (\tan(x))'
        &amp;=&amp;
        \left(\dfrac{\sin(x)}{\cos(x)}\right)' \\[1em]

        &amp;=&amp;
        \dfrac{\cos(x)\sin'(x)-\sin(x)\cos'(x)}{\cos^2(x)} \\[1em]

        &amp;=&amp;
        \dfrac{\cos(x)\cos(x)-\sin(x)(-\sin(x))}{\cos^2(x)} \\[1em]

        &amp;=&amp;
        \dfrac{\cos^2(x)+\sin^2(x)}{\cos^2(x)} \\[1em]

        &amp;=&amp;
        \dfrac{1}{\cos^2(x)} \\[1em]

        &amp;=&amp;
        \sec^2(x).
      \end{array}
    </me>

    <p>
      Therefore, <m>(\tan(x))'=\sec^2(x)</m> wherever <m>\tan(x)</m> is defined.
    </p>
  </proof>
</theorem>

<p>
  And similarly
</p>

<theorem xml:id="thm-derivative-sec-cot-csc">
  <statement>
    <p>
      For all real <m>x</m> such that the following functions are defined,
    </p>

    <me>
      \begin{array}{rcl}
        (\sec(x))' &amp;=&amp; \sec(x)\tan(x), \\[0.5em]
        (\cot(x))' &amp;=&amp; -\csc^2(x), \\[0.5em]
        (\csc(x))' &amp;=&amp; -\csc(x)\cot(x).
      \end{array}
    </me>
  </statement>
</theorem>

    <remark xml:id="rem-radians-warning">
      <p>
        Again remember, the derivative formulas in this section are valid when <m>x</m> is measured in <em>radians</em>, not degrees.
      </p>
    </remark>


  <p>
  Now let’s take a moment to incorporate this new knowledge into ideas from earlier sections before moving on to our discussion of limits.
</p>

<example xml:id="ex-derivative-sqrt-tan">

  <statement>
    <p>
      Find <m>f'(x)</m> if <m>f(x)=\sqrt{x}\tan(x)</m>.
    </p>
  </statement>

  <solution>
    <p>
      Since <m>f(x)</m> is written as a product of two functions, we apply the Product Rule.
    </p>
    
    <me>
      \begin{array}{rcl}
        f'(x)
        &amp;=&amp;
        \dfrac{1}{2\sqrt{x}}\tan(x)+\sqrt{x}\sec^2(x).
      \end{array}
    </me>

    <p>
      This expression is an acceptable final answer, though it could be simplified further if desired.
    </p>
  </solution>
</example>

<example xml:id="ex-derivative-cos-over-3x2">

  <statement>
    <p>
      Evaluate <m>\dfrac{d}{dx}\!\left(\dfrac{\cos(x)}{3x^2}\right)</m>.
    </p>
  </statement>

  <solution>
    <p>
      Since the function is written as a quotient, we apply the Quotient Rule.
    </p>

    <me>
      \begin{array}{rcl}
        \dfrac{d}{dx}\!\left(\dfrac{\cos(x)}{3x^2}\right)
        &amp;=&amp;
        \dfrac{(3x^2)(-\sin(x))-\cos(x)(6x)}{(3x^2)^2}\\[0.75em]

        &amp;=&amp;
        \dfrac{-3x^2\sin(x)-6x\cos(x)}{9x^4}\\[0.75em]

        &amp;=&amp;
        \dfrac{-x\sin(x)-2\cos(x)}{3x^3}.
      \end{array}
    </me>
  </solution>
</example>



  </subsection>


<subsection xml:id="foundational-trig-limits">
  <title>Two Fundamental Trigonometric Limits</title>

  <p>
    Previously in this section, we outlined the proof that the derivative of the sine function is the cosine function.
    That argument reduces to evaluating certain key limits involving sine and cosine as the input approaches zero.
    In this subsection, we formally establish those limits using a generic variable <m>u</m>.
    This prepares us for the substitutions and rewrites that commonly appear in trigonometric limit problems.
  </p>

  <theorem xml:id="thm-limit-sin-u-over-u">
    <statement>
      <p>
        <m>\displaystyle \lim_{u\to 0}\frac{\sin(u)}{u}=1</m>.
      </p>
    </statement>

    <proof>
      <p>
        Consider the unit circle and an angle <m>u</m> measured in radians, with <m>u \geq 0</m>.
        Geometric arguments<fn>
          This typically involves comparing the areas of triangles and circular sectors in the unit circle.
          In previous semesters, the full argument has been worked through in recitation.
          For students who are curious, Khan Academy also has a great video on this topic.
        </fn> show that
      </p>

      <me>
        \sin(u) \le u \le \tan(u).
      </me>

      <p>
        Dividing all three expressions by <m>\sin(u)</m> gives
      </p>

      <me>
        1 \le \frac{u}{\sin(u)} \le \frac{1}{\cos(u)}.
      </me>

      <p>
        Taking reciprocals reverses the inequalities:
      </p>

      <me>
        \cos(u) \le \frac{\sin(u)}{u} \le 1.
      </me>

      <p>
        As <m>u\to 0</m>, we know <m>\cos(u)\to 1</m>. Since
        <m>\frac{\sin(u)}{u}</m> is trapped between two expressions that both
        approach <m>1</m>, the Squeeze Theorem implies
      </p>

      <me>
        \lim_{u\to 0}\frac{\sin(u)}{u}=1.
      </me>
    </proof>
  </theorem>

  <theorem xml:id="thm-limit-cos-u-minus-one-over-u">
    <statement>
      <p>
        <m>\displaystyle \lim_{u\to 0}\frac{\cos(u)-1}{u}=0</m>.
      </p>
    </statement>

    <proof>
      <p>
        Rewrite the expression by multiplying the numerator and denominator
        by <m>\cos(u)+1</m>:
      </p>

      <me>
        \frac{\cos(u)-1}{u}
        =
        \frac{(\cos(u)-1)(\cos(u)+1)}{u(\cos(u)+1)}
        =
        \frac{-\sin^2(u)}{u(\cos(u)+1)}.
      </me>

      <p>
        Rewrite this expression to isolate the sine-over-input factor:
      </p>

      <me>
        \frac{-\sin^2(u)}{u(\cos(u)+1)}
        =
        -\left(\frac{\sin(u)}{u}\right)\left(\frac{\sin(u)}{\cos(u)+1}\right).
      </me>

      <p>
        As <m>u\to 0</m>, we have <m>\frac{\sin(u)}{u}\to 1</m>,
        <m>\sin(u)\to 0</m>, and <m>\cos(u)+1\to 2</m>.
        Therefore the entire product approaches <m>0</m>, and
      </p>

      <me>
        \lim_{u\to 0}\frac{\cos(u)-1}{u}=0.
      </me>
    </proof>
  </theorem>

  <p>
    These two limits supply the missing analytic step in the proof of the
    sine and cosine derivative formulas and will be used repeatedly to
    evaluate more complicated trigonometric limits.
  </p>
</subsection>




  <subsection xml:id="trig-limits-from-sin-over-x">
    <title>Limits of Trigonometric Quotients</title>

    <p>
      Many trigonometric limits can be evaluated by rewriting the expression until a factor of the form
      <m>\displaystyle \frac{\sin(u)}{u}</m> appears, where <m>u\to 0</m>.
      Then we use <m>\displaystyle \lim_{u\to 0}\frac{\sin(u)}{u}=1</m>.
    </p>

    <example xml:id="ex-limit-sin3x-over-x">
      <statement>
        <p>
          Compute <m>\displaystyle \lim_{x\to 0}\frac{\sin(3x)}{x}</m>.
        </p>
      </statement>

      <solution>
        <p>
          Multiply and divide by <m>3</m> to create <m>\displaystyle \frac{\sin(3x)}{3x}</m>.
        </p>

        <me>
\begin{array}{rcl}
\displaystyle \lim_{x\to 0}\frac{\sin(3x)}{x}
\amp=\amp \displaystyle \lim_{x\to 0}\left(\frac{\sin(3x)}{3x}\cdot \frac{3x}{x}\right)
\\[1.1em]
\amp=\amp \displaystyle \left(\lim_{x\to 0}\frac{\sin(3x)}{3x}\right)\left(\lim_{x\to 0}3\right)
\\[1.1em]
\amp=\amp \displaystyle \left(\lim_{u\to 0}\frac{\sin(u)}{u}\right)\cdot 3
\\[0.8em]
\amp=\amp \displaystyle 1\cdot 3
\\[0.6em]
\amp=\amp \displaystyle 3.
\end{array}
        </me>

        <p>
          In the third line we used the substitution <m>u=3x</m>, so <m>x\to 0</m> forces <m>u\to 0</m>.
        </p>
      </solution>
    </example>

    <example xml:id="ex-limit-tan-over-sin-sqrtx">
      <statement>
        <p>
          Compute <m>\displaystyle \lim_{x\to 0^+}\frac{\tan(x)}{\sin(\sqrt{x})}</m>.
        </p>
      </statement>

      <solution>
        <p>
          Rewrite <m>\tan(x)=\dfrac{\sin(x)}{\cos(x)}</m> and then introduce the standard sine-over-input factors.
        </p>

        <me>
\begin{array}{rcl}
\displaystyle \lim_{x\to 0^+}\frac{\tan(x)}{\sin(\sqrt{x})}
\amp=\amp \displaystyle \lim_{x\to 0^+}\left(\frac{\sin(x)}{\cos(x)}\cdot \frac{1}{\sin(\sqrt{x})}\right)
\\[1.1em]
\amp=\amp \displaystyle \lim_{x\to 0^+}\left(\frac{1}{\cos(x)}\cdot \frac{\sin(x)}{x}\cdot x \cdot \frac{\sqrt{x}}{\sin(\sqrt{x})}\cdot \frac{1}{\sqrt{x}}\right)
\\[1.3em]
\amp=\amp \displaystyle \lim_{x\to 0^+}\left(\frac{\sqrt{x}}{\cos(x)}\cdot \frac{\sin(x)}{x}\cdot \frac{1}{\frac{\sin(\sqrt{x})}{\sqrt{x}}}\right)
\\[1.3em]
\amp=\amp \displaystyle \frac{\sqrt{0}}{\cos(0)}\cdot 1\cdot \frac{1}{1}
\\[0.8em]
\amp=\amp \displaystyle 0.
\end{array}
        </me>

        <p>
          We used <m>\displaystyle \lim_{x\to 0}\frac{\sin(x)}{x}=1</m> and also
          <m>\displaystyle \lim_{x\to 0^+}\frac{\sin(\sqrt{x})}{\sqrt{x}}=1</m> by the substitution <m>u=\sqrt{x}</m>.
        </p>
      </solution>
    </example>
  </subsection>


<subsection xml:id="additional-worked-problems-derivTrig">
  <title>Additional Worked-Out Examples</title>

  <p>
    To keep this section at a reasonable length, we include only a few representative examples directly in the text.
    If you find yourself stuck on a homework problem, or if you are studying before a quiz or exam, additional
    fully worked-out examples are available via: 
    <alert>
      <xref ref="subsec-deriv-trig">
        Additional Examples for Trigonometric Derivatives
      </xref>
    </alert>
  </p>

</subsection>

  <exercises xml:id="exercises-derivative-trig-tf">
  <title>Practice / Study Problems</title>


    <exercisegroup>
      <title>True/False Questions</title>

      <introduction>
        <p>
          Determine whether each statement is true or false.
          Justify your answer.
        </p>


      </introduction>


    <exercise xml:id="tf-deriv-trig-07">
      <statement>
        <p>
          <m>\displaystyle \frac{d}{dx}(\cos(x))=\sin(x)</m>.
        </p>
      </statement>
    </exercise>


    <exercise xml:id="tf-deriv-trig-02">
      <statement>
        <p>
          If angles are measured in degrees, then <m>(\sin(x))'=\cos(x)</m>
          still holds without modification.
        </p>
      </statement>
    </exercise>


    

    



  <exercise xml:id="tf-deriv-trig-comp-01">
      <statement>
        <p>
          If <m>f(x)=\cos(x)\tan(x)</m>, then <m>f'(x)=\cos(x)</m>.
        </p>
      </statement>
      <solution>
        <p>
          <em>True.</em> We can use either algebra or the Product Rule.
          Since <m>\tan(x)=\dfrac{\sin(x)}{\cos(x)}</m> wherever it is defined,
        </p>
        <me>
          f(x)=\cos(x)\tan(x)=\cos(x)\cdot\frac{\sin(x)}{\cos(x)}=\sin(x)
        </me>
        <p>
          on the domain where <m>\tan(x)</m> is defined. Then
          <m>f'(x)=(\sin(x))'=\cos(x)</m>.
        </p>
        <p>
          Alternatively, using the Product Rule directly,
        </p>
        <me>
          \begin{array}{rcl}
            f'(x)
            &amp;=&amp;
            (\cos(x))'\tan(x)+\cos(x)(\tan(x))' \\[0.5em]
            &amp;=&amp;
            -\sin(x)\tan(x)+\cos(x)\sec^2(x) \\[0.5em]
            &amp;=&amp;
            -\sin(x)\dfrac{\sin(x)}{\cos(x)}+\cos(x)\dfrac{1}{\cos^2(x)} \\[0.5em]
            &amp;=&amp;
            =\dfrac{1-\sin^2(x)}{\cos(x)}
            =\dfrac{\cos^2(x)}{\cos(x)}=\cos(x).
          \end{array}
        </me>
      </solution>
    </exercise>

    <!-- 2. instantaneous rate of change at pi/2 -->

    <exercise xml:id="tf-deriv-trig-comp-02">
      <statement>
        <p>
          The instantaneous rate of change of <m>f(x)=x^2\sin(x)</m>
          at <m>x=\dfrac{\pi}{2}</m> is <m>\pi</m>.
        </p>
      </statement>
      <solution>
        <p>
          <em>True.</em> The instantaneous rate of change at a point is the derivative at that point.
          Use the Product Rule:
        </p>
        <me>
          \begin{array}{rcl}
            f'(x)
            &amp;=&amp;
            (x^2)'\sin(x)+x^2(\sin(x))' \\[0.5em]
            &amp;=&amp;
            2x\sin(x)+x^2\cos(x).
          \end{array}
        </me>
        <p>
          Evaluate at <m>x=\dfrac{\pi}{2}</m>:
        </p>
        <me>
          \begin{array}{rcl}
            f'\!\left(\dfrac{\pi}{2}\right)
            &amp;=&amp;
            2\cdot\dfrac{\pi}{2}\cdot\sin\!\left(\dfrac{\pi}{2}\right)
            +\left(\dfrac{\pi}{2}\right)^2\cos\!\left(\dfrac{\pi}{2}\right) \\[0.5em]
            &amp;=&amp;
            \pi\cdot 1 + \dfrac{\pi^2}{4}\cdot 0 \\[0.5em]
            &amp;=&amp;
            \pi.
          \end{array}
        </me>
        <p>
          So the instantaneous rate of change at <m>x=\dfrac{\pi}{2}</m> is <m>\pi</m>.
        </p>
      </solution>
    </exercise>

    <!-- 3. sec(x)/tan(x) at 0 -->

 <exercise xml:id="tf-deriv-trig-comp-03">
  <statement>
    <p>
      The slope of the tangent line to <m>f(x)=\dfrac{\csc(x)}{\cot(x)}</m>
      at <m>x=0</m> is <m>1</m>.
    </p>
  </statement>

  <solution>
    <p>
      <em>False.</em> First rewrite <m>f(x)</m> in simpler form.
      Since <m>\csc(x)=\dfrac{1}{\sin(x)}</m> and <m>\cot(x)=\dfrac{\cos(x)}{\sin(x)}</m>, we have
    </p>

    <me>
      f(x)
      =
      \frac{\csc(x)}{\cot(x)}
      =
      \frac{\dfrac{1}{\sin(x)}}{\dfrac{\cos(x)}{\sin(x)}}
      =
      \frac{1}{\cos(x)}
      =
      \sec(x),
    </me>

    <p>
      on any interval where the expressions are defined. Thus <m>f(x)=\sec(x)</m>.
    </p>

    <p>
      Now differentiate:
    </p>

    <me>
      f'(x) = (\sec(x))' = \sec(x)\tan(x).
    </me>

    <p>
      Evaluate at <m>x=0</m>:
    </p>

    <me>
      f'(0) = \sec(0)\tan(0) = 1 \cdot 0 = 0.
    </me>

    <p>
      The slope is <m>0</m>, not <m>1</m>, so the statement is false.
    </p>
  </solution>
</exercise>

<exercise xml:id="tf-deriv-trig-31">
  <statement>
    <p>
      Since <m>\displaystyle\frac{\sin(x)}{x}=1</m>, it follows that 
      <m>\displaystyle \left(\frac{\sin(x)}{x}\right)'=0</m>.
    </p>
  </statement>
<solution>
  <p>
    <em>False.</em> The equation <m>\sin(x)/x = 1</m> is <em>not</em> true for all <m>x</m>.
    The expression equals <m>1</m> only in the limiting sense 
    <m>\displaystyle \lim_{x\to 0}\frac{\sin(x)}{x}=1</m>, not as an identity.
    Since <m>\sin(x)/x</m> is not a constant function, its derivative is not zero.
    In fact, applying the Quotient Rule shows that 
    <m>\left(\dfrac{\sin(x)}{x}\right)'</m> is nonzero for all <m>x\neq 0</m>.
  </p>
</solution>

</exercise>




<exercise xml:id="tf-trig-limits-01">
  <statement>
    <p>
      <m>\displaystyle \lim_{x\to 0}\frac{\sin(x^2)}{x}=1</m>.
    </p>
  </statement>
  <solution>
    <p>
      <em>False.</em> Rewrite as 
      <m>\frac{\sin(x^2)}{x^2}\cdot x</m>.
      Since <m>\sin(u)/u → 1</m> as <m>u→0</m>, the product becomes <m>1·0 = 0</m>.
    </p>
  </solution>
</exercise>

<exercise xml:id="tf-trig-limits-02">
  <statement>
    <p>
      <m>\displaystyle \lim_{x\to 0}\frac{\cos(x)}{x}=1</m>.
    </p>
  </statement>
  <solution>
    <p>
      <em>False.</em> <m>\cos(x)/x</m> grows without bound as <m>x→0</m>.
      The limit does not exist as a finite number.
    </p>
  </solution>
</exercise>

<exercise xml:id="tf-trig-limits-03">
  <statement>
    <p>
      <m>\displaystyle \lim_{x\to 0}\frac{x}{\tan(3x)}=\dfrac13</m>.
    </p>
  </statement>
<solution>
  <p>
    <em>True.</em> Rewrite the expression to introduce the standard limit 
    <m>\displaystyle \lim_{u\to 0}\frac{\tan(u)}{u}=1</m>.
  </p>

  <md>
    <mrow>
      \lim_{x\to 0}\frac{x}{\tan(3x)}
      \amp=
      \lim_{x\to 0}\left(\frac{3x}{\tan(3x)}\cdot \frac{1}{3}\right)
    </mrow>

    <mrow>
      \amp=
      \left(\lim_{u\to 0}\frac{u}{\tan(u)}\right)\cdot \frac{1}{3}
      \quad \text{(using the substitution } u=3x\text{)}
    </mrow>

    <mrow>
      \amp=
      1\cdot \frac{1}{3}
    </mrow>

    <mrow>
      \amp=
      \frac{1}{3}.
    </mrow>
  </md>

  <p>
    Therefore the statement is true.
  </p>
</solution>

</exercise>



<exercise xml:id="tf-trig-limits-06">
  <statement>
    <p>
      <m>\displaystyle \lim_{x\to 0}\frac{\sin(5x)}{\sin(2x)}=\frac52</m>.
    </p>
  </statement>
  <solution>
    <p>
      <em>True.</em> Replace each term with <m>\sin(kx)/(kx)</m>:
      <m>\frac{\sin(5x)}{5x}\cdot\frac{2x}{\sin(2x)}\cdot \frac52 → 1·1·\frac52</m>.
    </p>
  </solution>
</exercise>

<exercise xml:id="tf-trig-limits-07">
  <statement>
    <p>
      <m>\displaystyle \lim_{x\to 0}\frac{\cos(x)-1}{\sin(x)}=0</m>.
    </p>
  </statement>
  <solution>
    <p>
      <em>True.</em> Use the identity 
      <m>\cos(x)-1 = -2\sin^2(x/2)</m>.
      Then the expression becomes 
      <m>-2\sin(x/2)\cdot\frac{\sin(x/2)}{\sin(x)}</m>, which tends to <m>0</m>.
    </p>
  </solution>
</exercise>



      </exercisegroup>
    </exercises>
 


</section>
