<?xml version="1.0" encoding="UTF-8"?>

<section xml:id="sec-derivative-rules" xmlns:xi="http://www.w3.org/2001/XInclude">
  <title>Basic Differentiation Rules</title>


  <objectives>
    <ul>
      <li>
        Interpret derivative notation in both Newton form <m>f'(x)</m> and Leibniz form <m>\displaystyle \frac{df}{dx}</m>.
      </li>
      <li>
        Use basic derivative formulas to differentiate power functions and constants.
      </li>
      <li>
        Apply the sum, constant multiple, product, and quotient rules to compute derivatives algebraically.
      </li>
      <li>
        Interpret higher derivatives in an applied context (velocity and acceleration).
      </li>
    </ul>
  </objectives>

  <p>
    So far, we have seen how real-world rate-of-change problems and geometric tangent-line problems lead to derivatives.
    In this section, we focus on computing derivatives efficiently by using algebraic rules, so we do not need to return to the limit definition every time.
  </p>

  <subsection xml:id="derivative-notation">
    <title>Notation for the Derivative</title>

    <p>
      The derivative of a function <m>f</m> can be written in several equivalent ways. In Newton notation we write <m>f'(x)</m>.
      In Leibniz notation we write <m>\displaystyle \frac{df}{dx}</m>, which is meant to remind us of the definition of the derivative as a limit of difference quotients:
    </p>

    <me>
      \displaystyle f'(x)=\frac{df}{dx}=\lim_{\Delta x\to 0}\frac{\Delta f}{\Delta x}.
    </me>

    <p>
      Here <m>\Delta x</m> is a change in the input, and <m>\Delta f</m> is the corresponding change in the output:
      <m>\Delta x=h</m> and <m>\Delta f=f(x+h)-f(x)</m>.
      The notation <m>\displaystyle \frac{df}{dx}</m> does <emph>not</emph> literally mean “a quotient of two tiny numbers.”
      It is a single symbol that represents a limit.
    </p>

    <p>
      For example, if <m>f(x)=x^2</m>, then the derivative formula <m>f'(x)=2x</m> can be written as
    </p>

    <me>
      \displaystyle \frac{d}{dx}(x^2)=2x.
    </me>

    <p>
      To emphasize the difference between “the derivative function” and “the derivative at a point,” we write
      <m>\displaystyle f'(a)=\left.\frac{df}{dx}\right|_{x=a}</m>.
      You may also see the notation <m>Df</m> for the derivative of <m>f</m>, so that <m>f'(x)=Df(x)</m>.
    </p>
  </subsection>

  <subsection xml:id="basic-derivatives">
    <title>Basic Derivatives</title>

    <p>
      The strategy is the same as earlier limit techniques: we establish derivatives of basic functions, then build more complicated derivatives from those.
      The most important basic formulas are the following.
    </p>

<theorem xml:id="thm-constant-and-linear-derivatives">
  <title>Derivatives of Constant and Linear Functions</title>
  <statement>
    <ul>
      <li>
        If <m>f(x) = c</m> is a constant function, then
        <m>\displaystyle \frac{d}{dx}(c) = 0</m>.
      </li>
      <li>
        If <m>f(x) = x</m>, then
        <m>\displaystyle \frac{d}{dx}(x) = 1</m>.
      </li>
    </ul>
  </statement>
  <proof>
  <p>
    We use the limit definition of the derivative.
  </p>

  <p>
    First, suppose <m>f(x) = c</m>, where <m>c</m> is a constant.
    By definition,
  </p>

  <me>
    \displaystyle
    \frac{d}{dx}(c)
    =
    \lim_{h \to 0} \frac{f(x+h) - f(x)}{h}.
  </me>

  <p>
    Since <m>f(x+h) = c</m> and <m>f(x) = c</m>, the numerator is zero.
  </p>

  <me>
    \displaystyle
    \frac{d}{dx}(c)
    =
    \lim_{h \to 0} \frac{c - c}{h}
    =
    \lim_{h \to 0} \frac{0}{h}
    =
    0.
  </me>

  <p>
    Therefore, the derivative of a constant function is zero.
  </p>

  <p>
    Next, suppose <m>f(x) = x</m>.
    Using the limit definition,
  </p>

  <me>
    \displaystyle
    \frac{d}{dx}(x)
    =
    \lim_{h \to 0} \frac{(x+h) - x}{h}.
  </me>

  <p>
    Simplifying the numerator gives
  </p>

  <me>
    \displaystyle
    \frac{d}{dx}(x)
    =
    \lim_{h \to 0} \frac{h}{h}
    =
    \lim_{h \to 0} 1
    =
    1.
  </me>

  <p>
    Therefore, the derivative of <m>f(x) = x</m> is equal to <m>1</m>.
  </p>

</proof>

</theorem>

<theorem xml:id="thm-power-rule">
  <title>The Power Rule</title>
  <statement>
    <p>
      Let <m>p</m> be any real number for which <m>x^p</m> is defined.
      If <m>f(x) = x^p</m>, then
    </p>
    <me>
      \displaystyle \frac{d}{dx}(x^p) = p x^{p-1}.
    </me>
  </statement>
<proof>
  <p>
    We begin with a geometric intuition.
    For the function <m>f(x)=x^2</m>, increasing <m>x</m> by a small amount
    <m>h = \Delta x</m> produces a change in area
    <m>\Delta f</m> that is approximately <m>2x\,\Delta x</m>.
  </p> 
  <sidebyside width="80%">
    <figure xml:id="xSquareProof">
      <caption>
        A secant line connecting the points <m>(1,f(1))</m> and <m>(7,f(7))</m>,
        representing the average rate of change of <m>f</m> on the interval <m>[1,7]</m>.
      </caption>
      <image source="images/xSquareDerivProof.png" width="100%"/>
    </figure>
  </sidebyside>

<p>
    This suggests that
  </p>

  <me>
    f'(x) \approx \frac{\Delta f}{\Delta x} \approx 2x.
  </me>

  <p>
    A similar idea applies to volume.
    For <m>f(x)=x^3</m>, the change in volume due to a small increase
    <m>\Delta x</m> is approximately <m>3x^2\,\Delta x</m>, </p>
  <sidebyside width="80%">
    <figure xml:id="xCubeProof">
      <caption>
        A secant line connecting the points <m>(1,f(1))</m> and <m>(7,f(7))</m>,
        representing the average rate of change of <m>f</m> on the interval <m>[1,7]</m>.
      </caption>
      <image source="images/xCubeDerivProof.png" width="100%"/>
    </figure>
  </sidebyside>
    <p> 
    suggesting that <m>f'(x) \approx 3x^2</m>.
  </p>

  <p>
    More generally, for the growth of an <m>n</m>-dimensional cube with side length <m>x</m>,
    this geometric reasoning suggests that
    <m>f'(x)=n x^{n-1}</m>.
    While this intuition cannot be visualized for higher dimensions,
    it motivates the algebraic proof that follows.
  </p>

  <p>
    We now prove the Power Rule rigorously using the limit definition of the derivative.
    The constant and linear cases were proved earlier.
    We focus on the case
    <m>f(x)=x^p</m>.
  </p>

  <p>
    The proof proceeds in stages, beginning with whole number powers.
    Throughout, we repeatedly use the identity
  </p>

  <me>
    a^n - b^n
    =
    (a-b)\big(a^{n-1}+a^{n-2}b+a^{n-3}b^2+\cdots+b^{n-1}\big),
  </me>

  <p>
    which holds for all positive integers <m>n</m>.
  </p>

  <p>
    <em>Step 1: Positive integer powers.</em>
    Let <m>p=n</m> be a positive integer.
    Using the limit definition of the derivative,
  </p>

  <me>
    \displaystyle
    \frac{d}{dx}(x^n)
    =
    \lim_{h\to 0}\frac{(x+h)^n-x^n}{h}.
  </me>

  <p>
    Apply the factorization identity with <m>a=x+h</m> and <m>b=x</m>.
  </p>

  <me>
    \displaystyle
    \frac{(x+h)^n-x^n}{h}
    =
    \frac{(x+h-x)\big((x+h)^{n-1}+(x+h)^{n-2}x+\cdots+x^{n-1}\big)}{h}.
  </me>

  <p>
    Cancel the factor of <m>h</m> to obtain
  </p>

  <me>
    \displaystyle
    (x+h)^{n-1}+(x+h)^{n-2}x+\cdots+x^{n-1}.
  </me>

  <p>
    Taking the limit as <m>h\to 0</m> gives
  </p>

  <me>
    \displaystyle
    x^{n-1}+x^{n-1}+\cdots+x^{n-1}
    =
    n x^{n-1}.
  </me>

  <p>
    Therefore, for positive integers <m>n</m>,
  </p>

  <me>
    \displaystyle
    \frac{d}{dx}(x^n)=n x^{n-1}.
  </me>

  <p>
    <em>Step 2: Negative integer powers.</em>
    Let <m>p=-n</m>, where <m>n</m> is a positive integer.
    Then <m>x^p=\frac{1}{x^n}</m>.
    In the derivative limit, we combine fractions and apply the same
    factorization identity with <m>a=x</m> and <m>b=x+h</m>.
  </p>

  <p>
    After simplification, the resulting expression reduces to
  </p>

  <me>
    \displaystyle
    -\frac{n x^{n-1}}{x^{2n}}
    =
    (-n)x^{-n-1}.
  </me>

  <p>
    Thus, the Power Rule holds for negative integers as well.
  </p>

  <p>
    <em>Step 3: Rational powers.</em>
    Let <m>p=\frac{n}{m}</m>, where <m>m</m> is a positive integer
    and <m>n</m> is any integer.
    Then
  </p>

  <me>
    x^p = x^{n/m} = \sqrt[m]{x^n}.
  </me>

  <p>
    In the derivative limit, the numerator has the form
    <m>\sqrt[m]{(x+h)^n}-\sqrt[m]{x^n}</m>.
    As in earlier work with cube roots,
    we multiply the numerator and denominator by
  </p>

  <me>
    a^{m-1}+a^{m-2}b+\cdots+b^{m-1},
  </me>

  <p>
    where <m>a=\sqrt[m]{(x+h)^n}</m> and <m>b=\sqrt[m]{x^n}</m>.
    This eliminates the radicals and produces the numerator
  </p>

  <me>
    a^m-b^m=(x+h)^n-x^n,
  </me>

  <p>
    which we have already handled.
    Simplifying the resulting limit again yields
    <m>p x^{p-1}</m>.
  </p>

  <p>
    Therefore, the Power Rule holds for all rational exponents.
  </p>

  <p>
    The formula
    <m>\frac{d}{dx}(x^p)=p x^{p-1}</m>
    is also valid for irrational exponents such as <m>p=\sqrt{2}</m>,
    but proving this rigorously requires more advanced theory.
  </p>
</proof>
</theorem>




    <example xml:id="ex-basic-derivatives-examples">
      <statement>
        <p>
          Use the power rule to compute each derivative.
        </p>
        <ol>
          <li><m>\displaystyle \frac{d}{dx}(x^{10})</m></li>
          <li><m>\displaystyle \frac{d}{dx}\!\left(\sqrt[3]{x}\right)</m></li>
          <li><m>\displaystyle \frac{d}{dx}\!\left(\frac{1}{x}\right)</m></li>
        </ol>
      </statement>

      <solution>
        <p>
          Rewrite roots and reciprocals using exponents, then apply <m>\displaystyle \frac{d}{dx}(x^p)=px^{p-1}</m>.
        </p>

        <me>
\begin{array}{rcl}
\displaystyle \frac{d}{dx}(x^{10})
\amp=\amp \displaystyle 10x^{9},
\\[0.8em]
\displaystyle \frac{d}{dx}\!\left(\sqrt[3]{x}\right)
\amp=\amp \displaystyle \frac{d}{dx}\!\left(x^{1/3}\right)
= \frac{1}{3}x^{-2/3}
= \frac{1}{3\sqrt[3]{x^2}},
\\[0.8em]
\displaystyle \frac{d}{dx}\!\left(\frac{1}{x}\right)
\amp=\amp \displaystyle \frac{d}{dx}\!\left(x^{-1}\right)
= -x^{-2}
= -\frac{1}{x^2}.
\end{array}
        </me>
      </solution>
    </example>
  </subsection>

  <subsection xml:id="derivative-rules">
    <title>Derivative Rules</title>

    <p>
      Once we know the derivatives of basic functions, we can differentiate combinations of functions using rules.
      Suppose <m>f</m> and <m>g</m> are differentiable at <m>x</m>.
    </p>

    <theorem xml:id="thm-derivative-rules">
      <statement>
        <ul>
          <li>
            <emph>Sum Rule:</emph> <m>\displaystyle (f(x)+g(x))'=f'(x)+g'(x)</m>.
          </li>
          <li>
            <emph>Difference Rule:</emph> <m>\displaystyle (f(x)-g(x))'=f'(x)-g'(x)</m>.
          </li>
          <li>
            <emph>Constant Multiple Rule:</emph> <m>\displaystyle (c\,f(x))'=c\,f'(x)</m> for any constant <m>c</m>.
          </li>
          <li>
            <emph>Product Rule:</emph> <m>\displaystyle (f(x)g(x))'=f'(x)g(x)+f(x)g'(x)</m>.
          </li>
          <li>
            <emph>Quotient Rule:</emph>
            <m>\displaystyle \left(\frac{f(x)}{g(x)}\right)'=\frac{f'(x)g(x)-f(x)g'(x)}{g(x)^2}</m>, where <m>g(x)\neq 0</m>.
          </li>
        </ul>
      </statement>
    </theorem>

    <remark xml:id="rem-product-warning">
      <p>
        Warning: the derivative of a product is <emph>not</emph> the product of derivatives.
        In general, <m>\displaystyle (f(x)g(x))'\neq f'(x)g'(x)</m>.
      </p>
    </remark>

    <example xml:id="ex-sum-rule-proof">
      <statement>
        <p>
          Use the definition of the derivative to justify the Sum Rule:
          <m>\displaystyle (f(x)+g(x))'=f'(x)+g'(x)</m>.
        </p>
      </statement>

      <solution>
        <p>
          Start with the limit definition and separate the difference quotient into two pieces:
        </p>

        <me>
\begin{array}{rcl}
\displaystyle (f(x)+g(x))'
\amp=\amp \displaystyle \lim_{h\to 0}\frac{(f(x+h)+g(x+h))-(f(x)+g(x))}{h}
\\[1.1em]
\amp=\amp \displaystyle \lim_{h\to 0}\left(\frac{f(x+h)-f(x)}{h}+\frac{g(x+h)-g(x)}{h}\right)
\\[1.1em]
\amp=\amp \displaystyle \lim_{h\to 0}\frac{f(x+h)-f(x)}{h}
+\lim_{h\to 0}\frac{g(x+h)-g(x)}{h}
\\[1.1em]
\amp=\amp \displaystyle f'(x)+g'(x).
\end{array}
        </me>

        <p>
          This step uses limit laws for sums.
        </p>
      </solution>
    </example>

    <p>
      The Product Rule can be motivated geometrically using an area model for a rectangle with side lengths <m>f(x)</m> and <m>g(x)</m>.
    </p>

    <figure xml:id="fig-product-rule-rectangle">
      <caption>
        A geometric picture behind the Product Rule: the change in area comes from two edge strips plus a tiny corner piece.
      </caption>
      <image source="2-3-Rect-1.png" width="70%"/>
    </figure>

    <remark xml:id="rem-product-rule-idea">
      <p>
        When <m>\Delta x=h</m> is small, the changes <m>\Delta f</m> and <m>\Delta g</m> are small as well.
        The change in area is
        <m>\Delta(f\cdot g)=(\Delta f)\,g(x)+f(x)(\Delta g)+(\Delta f)(\Delta g)</m>.
        After dividing by <m>\Delta x</m> and taking <m>\Delta x\to 0</m>, the term involving <m>(\Delta f)(\Delta g)</m> vanishes,
        producing <m>\displaystyle (fg)'=f'g+fg'</m>.
      </p>
    </remark>
  </subsection>

  <subsection xml:id="derivative-computations">
    <title>Derivative Computations</title>

    <example xml:id="ex-derivative-sqrtx">
      <statement>
        <p>
          Compute <m>\displaystyle \frac{d}{dx}(\sqrt{x})</m>.
        </p>
      </statement>
      <solution>
        <p>
          Write <m>\sqrt{x}=x^{1/2}</m> and use the power rule.
        </p>

        <me>
\begin{array}{rcl}
\displaystyle \frac{d}{dx}(\sqrt{x})
\amp=\amp \displaystyle \frac{d}{dx}(x^{1/2})
\\[0.8em]
\amp=\amp \displaystyle \frac{1}{2}x^{-1/2}
\\[0.8em]
\amp=\amp \displaystyle \frac{1}{2\sqrt{x}}.
\end{array}
        </me>
      </solution>
    </example>

    <example xml:id="ex-derivative-constant">
      <statement>
        <p>
          Compute <m>\displaystyle \frac{d}{dx}(\sqrt{10})</m>.
        </p>
      </statement>
      <solution>
        <p>
          <m>\sqrt{10}</m> is a constant, so its derivative is <m>0</m>.
        </p>
      </solution>
    </example>

    <example xml:id="ex-product-rule-algebra">
      <statement>
        <p>
          Let <m>f(x)=(5x^2+1)(\sqrt{x}-3)</m>. Compute <m>f'(x)</m>.
        </p>
      </statement>
      <solution>
        <p>
          Use the Product Rule with <m>u(x)=5x^2+1</m> and <m>v(x)=\sqrt{x}-3</m>.
        </p>

        <me>
\begin{array}{rcl}
\displaystyle f'(x)
\amp=\amp \displaystyle u'(x)v(x)+u(x)v'(x)
\\[0.9em]
\amp=\amp \displaystyle (10x)(\sqrt{x}-3)+(5x^2+1)\left(\frac{1}{2\sqrt{x}}\right).
\end{array}
        </me>

        <p>
          (Optional) You can also expand first and then differentiate term-by-term. Both approaches agree.
        </p>
      </solution>
    </example>

    <example xml:id="ex-quotient-rule-two-ways">
      <statement>
        <p>
          Differentiate <m>g(t)=\dfrac{t^5+1}{t\sqrt{t}}</m>.
        </p>
      </statement>

      <solution>
        <p>
          First rewrite the denominator: <m>t\sqrt{t}=t^{3/2}</m>. Then
          <m>\displaystyle g(t)=(t^5+1)t^{-3/2}=t^{7/2}+t^{-3/2}</m>, so
        </p>

        <me>
\begin{array}{rcl}
\displaystyle g'(t)
\amp=\amp \displaystyle \frac{d}{dt}\left(t^{7/2}+t^{-3/2}\right)
\\[0.9em]
\amp=\amp \displaystyle \frac{7}{2}t^{5/2}-\frac{3}{2}t^{-5/2}.
\end{array}
        </me>

        <p>
          You could also use the Quotient Rule directly; both methods produce equivalent results.
        </p>
      </solution>
    </example>

    <example xml:id="ex-ice-block-volume">
      <statement>
        <p>
          A block of ice has length <m>\ell=10</m> cm, width <m>w=5</m> cm, and height <m>h=20</m> cm.
          Its length and width are decreasing at <m>1</m> cm/hr, and its height is decreasing at <m>2</m> cm/hr.
          How fast is the volume decreasing at that instant?
        </p>
      </statement>

      <solution>
        <p>
          The volume is <m>V=\ell w h</m>, and all three dimensions depend on time <m>t</m>.
          Differentiate using the Product Rule (applied twice):
        </p>

        <me>
\begin{array}{rcl}
\displaystyle \frac{dV}{dt}
\amp=\amp \displaystyle \frac{d}{dt}(\ell w h)
\\[0.8em]
\amp=\amp \displaystyle \ell'wh+\ell w'h+\ell w h'.
\end{array}
        </me>

        <p>
          At the instant described:
          <m>\ell=10</m>, <m>w=5</m>, <m>h=20</m>,
          <m>\ell'=-1</m>, <m>w'=-1</m>, <m>h'=-2</m> (cm/hr).
        </p>

        <me>
\begin{array}{rcl}
\displaystyle \frac{dV}{dt}
\amp=\amp \displaystyle (-1)(5)(20)+(10)(-1)(20)+(10)(5)(-2)
\\[0.8em]
\amp=\amp \displaystyle -100-200-100
\\[0.8em]
\amp=\amp \displaystyle -400.
\end{array}
        </me>

        <p>
          The volume is decreasing at <m>400</m> cm<sup>3</sup>/hr.
        </p>
      </solution>
    </example>
  </subsection>

  <subsection xml:id="higher-derivatives">
    <title>Higher Derivatives</title>

    <p>
      Because the derivative of a function is itself a function, we can differentiate again.
      The second derivative of <m>f</m> is denoted <m>f''(x)</m>, and in Leibniz notation it is written
      <m>\displaystyle \frac{d^2f}{dx^2}</m>:
    </p>

    <me>
      \displaystyle f''(x)=\frac{d}{dx}\!\left(f'(x)\right)=\frac{d}{dx}\!\left(\frac{df}{dx}\right)=\frac{d^2f}{dx^2}.
    </me>

    <p>
      If <m>f</m> represents position as a function of time, then <m>f'(t)</m> is velocity and <m>f''(t)</m> is acceleration.
    </p>

    <example xml:id="ex-higher-derivatives-falling-stone">
      <statement>
        <p>
          A stone falls <m>f(t)=16t^2</m> feet in <m>t</m> seconds. Compute <m>f'(t)</m>, <m>f''(t)</m>, and interpret them.
        </p>
      </statement>

      <solution>
        <p>
          Differentiate repeatedly using the power rule:
        </p>

        <me>
\begin{array}{rcl}
\displaystyle f'(t)
\amp=\amp \displaystyle (16t^2)'
=32t,
\\[0.8em]
\displaystyle f''(t)
\amp=\amp \displaystyle (32t)'
=32,
\\[0.8em]
\displaystyle f'''(t)
\amp=\amp \displaystyle (32)'
=0.
\end{array}
        </me>

        <p>
          Here <m>f'(t)=32t</m> is velocity (ft/sec), increasing with time.
          The constant <m>f''(t)=32</m> is acceleration (ft/sec<sup>2</sup>), and <m>f'''(t)=0</m> means the acceleration is not changing.
        </p>
      </solution>
    </example>

  </subsection>

</section>
