<?xml version="1.0" encoding="UTF-8"?>

<section xml:id="sec-derivative-implicit" xmlns:xi="http://www.w3.org/2001/XInclude">
  <title>Implicit Differentiation</title>

  <objectives>
    <ul>
      <li>Students should know when they should apply implicit differentiation.</li>
      <li>
        Students should be able to apply the implicit differentiation technique in simple to slightly complicated problems,
        including those requiring the use of the product, quotient, or chain rule.
      </li>
      <li>Students should be able to interpret the results of implicit differentiation as the slope of a curve.</li>
    </ul>
  </objectives>

  <subsection xml:id="implicit-diff-definition">
    <title>Key Idea: Implicit Differentiation</title>

    <definition xml:id="def-implicit-differentiation">
      <title>Implicit Differentiation</title>
      <statement>
        <p>
          <term>Implicit differentiation</term> consists of differentiating both sides of an equation with respect to <m>x</m>
          and then solving the resulting equation for <m>y'</m>.
        </p>
        <p>
          In the examples and exercises of this section, it is assumed that the given equation determines <m>y</m> implicitly
          as a differentiable function of <m>x</m>, so that implicit differentiation applies.
        </p>
      </statement>
    </definition>

    <remark xml:id="rem-implicit-why">
      <p>
        The key feature is that <m>y</m> depends on <m>x</m>, even if the equation does not explicitly solve for <m>y</m>.
        So whenever you differentiate an expression containing <m>y</m>, you must use the Chain Rule and include a factor of <m>y'</m>.
      </p>
    </remark>
  </subsection>

  <subsection xml:id="implicit-diff-straightforward">
    <title>Straightforward Examples</title>

    <example xml:id="ex-implicit-ln">
      <title>Implicit Differentiation with a Logarithm</title>
      <statement>
        <p>
          Given the equation <m>x\ln(y)+y^2=4x</m>, find <m>\displaystyle \frac{dy}{dx}</m> using implicit differentiation.
        </p>
      </statement>

      <solution>
        <p>
          Differentiate both sides with respect to <m>x</m>. The left side requires the Product Rule on <m>x\ln(y)</m>
          and the Chain Rule on <m>\ln(y)</m> and <m>y^2</m>.
        </p>

        <me>
\begin{array}{rcl}
\displaystyle \frac{d}{dx}\bigl(x\ln(y)\bigr)+\frac{d}{dx}\bigl(y^2\bigr)
\amp=\amp \displaystyle \frac{d}{dx}(4x)
\\[1.2em]
\displaystyle \Bigl(1\cdot \ln(y)+x\cdot \frac{1}{y}\,y'\Bigr)+2y\,y'
\amp=\amp \displaystyle 4.
\end{array}
        </me>

        <p>
          Now solve for <m>y'</m> by collecting terms with <m>y'</m>.
        </p>

        <me>
\begin{array}{rcl}
\displaystyle \frac{x}{y}\,y'+2y\,y'
\amp=\amp \displaystyle 4-\ln(y)
\\[1.2em]
\displaystyle y'\left(\frac{x}{y}+2y\right)
\amp=\amp \displaystyle 4-\ln(y)
\\[1.2em]
\displaystyle y'
\amp=\amp \displaystyle \frac{4-\ln(y)}{\frac{x}{y}+2y}.
\end{array}
        </me>

        <p>
          A common simplification is to multiply top and bottom by <m>y</m>:
        </p>

        <me>
          \displaystyle y'=\frac{y(4-\ln(y))}{x+2y^2}.
        </me>
      </solution>
    </example>

    <example xml:id="ex-implicit-astroid-like">
      <title>Horizontal Tangent in the First Quadrant</title>
      <statement>
        <p>
          Find <m>y'</m> if <m>y^3+x^3=6xy</m>. At what point in the first quadrant is the tangent line to this curve horizontal?
        </p>
      </statement>

      <solution>
        <p>
          Differentiate both sides with respect to <m>x</m>. On the right side, use the Product Rule on <m>6xy</m>.
        </p>

        <me>
\begin{array}{rcl}
\displaystyle \frac{d}{dx}(y^3)+\frac{d}{dx}(x^3)
\amp=\amp \displaystyle \frac{d}{dx}(6xy)
\\[1.2em]
\displaystyle 3y^2y'+3x^2
\amp=\amp \displaystyle 6\bigl(xy'+y\bigr)
\\[1.2em]
\displaystyle 3y^2y'+3x^2
\amp=\amp \displaystyle 6xy'+6y.
\end{array}
        </me>

        <p>
          Solve for <m>y'</m>.
        </p>

        <me>
\begin{array}{rcl}
\displaystyle 3y^2y'-6xy'
\amp=\amp \displaystyle 6y-3x^2
\\[1.2em]
\displaystyle y'(3y^2-6x)
\amp=\amp \displaystyle 3(2y-x^2)
\\[1.2em]
\displaystyle y'
\amp=\amp \displaystyle \frac{3(2y-x^2)}{3y^2-6x}
\ =\ \frac{2y-x^2}{y^2-2x}.
\end{array}
        </me>

        <p>
          A horizontal tangent occurs when <m>\displaystyle y'=0</m>, which requires the numerator to be zero (and the denominator nonzero):
        </p>

        <me>
          \displaystyle 2y-x^2=0 \quad\Longrightarrow\quad y=\frac{x^2}{2}.
        </me>

        <p>
          Substitute <m>\displaystyle y=\frac{x^2}{2}</m> into the original equation <m>y^3+x^3=6xy</m>.
        </p>

        <me>
\begin{array}{rcl}
\displaystyle \left(\frac{x^2}{2}\right)^3+x^3
\amp=\amp \displaystyle 6x\left(\frac{x^2}{2}\right)
\\[1.2em]
\displaystyle \frac{x^6}{8}+x^3
\amp=\amp \displaystyle 3x^3
\\[1.2em]
\displaystyle \frac{x^6}{8}
\amp=\amp \displaystyle 2x^3.
\end{array}
        </me>

        <p>
          In the first quadrant, <m>x&gt;0</m>, so divide by <m>x^3</m>:
        </p>

        <me>
\begin{array}{rcl}
\displaystyle \frac{x^3}{8}
\amp=\amp \displaystyle 2
\\[0.8em]
\displaystyle x^3
\amp=\amp \displaystyle 16
\\[0.8em]
\displaystyle x
\amp=\amp \displaystyle \sqrt[3]{16}.
\end{array}
        </me>

        <p>
          Then
          <m>\displaystyle y=\frac{x^2}{2}=\frac{(\sqrt[3]{16})^2}{2}=\frac{\sqrt[3]{256}}{2}</m>.
          So the point in the first quadrant where the tangent is horizontal is
        </p>

        <me>
          \displaystyle \left(\sqrt[3]{16},\,\frac{(\sqrt[3]{16})^2}{2}\right).
        </me>

        <p>
          (This point is valid as long as <m>y^2-2x\neq 0</m>, which you can check holds here.)
        </p>
      </solution>
    </example>

    <example xml:id="ex-implicit-tangent-line">
      <title>Tangent Line from an Implicit Equation</title>
      <statement>
        <p>
          Find an equation of the tangent line to the curve <m>y e^{\sin x}=x\cos y</m> at the point <m>(0,0)</m>.
        </p>
      </statement>

      <solution>
        <p>
          Differentiate both sides with respect to <m>x</m>. Use the Product Rule on both sides.
        </p>

        <me>
\begin{array}{rcl}
\displaystyle \frac{d}{dx}\bigl(ye^{\sin x}\bigr)
\amp=\amp \displaystyle \frac{d}{dx}\bigl(x\cos y\bigr)
\\[1.4em]
\displaystyle y'e^{\sin x}+y\cdot e^{\sin x}\cdot(\cos x)
\amp=\amp \displaystyle 1\cdot \cos y + x\cdot \frac{d}{dx}(\cos y)
\\[1.4em]
\displaystyle y'e^{\sin x}+y e^{\sin x}\cos x
\amp=\amp \displaystyle \cos y + x\cdot\bigl(-\sin y\bigr)\,y'.
\end{array}
        </me>

        <p>
          Now substitute <m>(x,y)=(0,0)</m>. Note <m>\sin(0)=0</m>, <m>e^0=1</m>, <m>\cos(0)=1</m>, and <m>\sin(0)=0</m>.
        </p>

        <me>
\begin{array}{rcl}
\displaystyle y'(1)+0
\amp=\amp \displaystyle 1+0
\\[0.8em]
\displaystyle y'
\amp=\amp \displaystyle 1.
\end{array}
        </me>

        <p>
          The slope at <m>(0,0)</m> is 1, so the tangent line is
        </p>

        <me>
          \displaystyle y=x.
        </me>
      </solution>
    </example>
  </subsection>

  <subsection xml:id="implicit-diff-conceptual">
    <title>More Challenging and Conceptual Problems</title>

    <example xml:id="ex-intercepts-tangent">
      <title>Intercept Form and a Constant Sum</title>
      <statement>
        <p>
          Show that the sum of the <m>x</m>- and <m>y</m>-intercepts of any tangent line to the curve
          <m>\sqrt{x}+\sqrt{y}=\sqrt{c}</m> is equal to <m>c</m>.
        </p>
      </statement>

      <solution>
        <p>
          Differentiate implicitly:
        </p>

        <me>
\begin{array}{rcl}
\displaystyle \frac{d}{dx}\bigl(\sqrt{x}\bigr)+\frac{d}{dx}\bigl(\sqrt{y}\bigr)
\amp=\amp \displaystyle \frac{d}{dx}\bigl(\sqrt{c}\bigr)
\\[1.2em]
\displaystyle \frac{1}{2\sqrt{x}}+\frac{1}{2\sqrt{y}}\,y'
\amp=\amp \displaystyle 0
\\[1.2em]
\displaystyle y'
\amp=\amp \displaystyle -\frac{\sqrt{y}}{\sqrt{x}}.
\end{array}
        </me>

        <p>
          At a point <m>(a,b)</m> on the curve, the slope is
          <m>\displaystyle m=-\frac{\sqrt{b}}{\sqrt{a}}</m>.
          The tangent line is
          <m>\displaystyle y-b=m(x-a)</m>.
        </p>

        <p>
          Find the intercepts. The <m>x</m>-intercept occurs when <m>y=0</m>:
        </p>

        <me>
\begin{array}{rcl}
\displaystyle 0-b
\amp=\amp \displaystyle m(x-a)
\\[0.8em]
\displaystyle x
\amp=\amp \displaystyle a-\frac{b}{m}
\ =\ a+b\frac{\sqrt{a}}{\sqrt{b}}
\ =\ a+\sqrt{ab}.
\end{array}
        </me>

        <p>
          So the <m>x</m>-intercept is <m>a+\sqrt{ab}</m>. The <m>y</m>-intercept occurs when <m>x=0</m>:
        </p>

        <me>
\begin{array}{rcl}
\displaystyle y-b
\amp=\amp \displaystyle m(0-a)
\\[0.8em]
\displaystyle y
\amp=\amp \displaystyle b-am
\ =\ b+a\frac{\sqrt{b}}{\sqrt{a}}
\ =\ b+\sqrt{ab}.
\end{array}
        </me>

        <p>
          Thus the sum of intercepts is
          <m>\displaystyle (a+\sqrt{ab})+(b+\sqrt{ab})=a+b+2\sqrt{ab}=(\sqrt{a}+\sqrt{b})^2</m>.
        </p>

        <p>
          Since <m>(a,b)</m> lies on <m>\sqrt{x}+\sqrt{y}=\sqrt{c}</m>, we have <m>\sqrt{a}+\sqrt{b}=\sqrt{c}</m>, so
          <m>(\sqrt{a}+\sqrt{b})^2=c</m>. Therefore the sum of the intercepts is always <m>c</m>.
        </p>
      </solution>
    </example>

    <example xml:id="ex-ellipse-parallel">
      <title>Parallel Tangents on an Ellipse</title>
      <statement>
        <p>
          Consider the ellipse given by <m>x^2-xy+y^2=3</m>. Find the points where the ellipse crosses the <m>x</m>-axis
          and show that the tangent lines at these points are parallel.
        </p>
      </statement>

      <solution>
        <p>
          Points on the <m>x</m>-axis have <m>y=0</m>. Substitute into the equation:
        </p>

        <me>
\begin{array}{rcl}
\displaystyle x^2-x(0)+0^2
\amp=\amp \displaystyle 3
\\[0.8em]
\displaystyle x^2
\amp=\amp \displaystyle 3
\\[0.8em]
\displaystyle x
\amp=\amp \displaystyle \pm \sqrt{3}.
\end{array}
        </me>

        <p>
          So the ellipse crosses the <m>x</m>-axis at <m>(\sqrt{3},0)</m> and <m>(-\sqrt{3},0)</m>.
        </p>

        <p>
          Differentiate implicitly:
        </p>

        <me>
\begin{array}{rcl}
\displaystyle \frac{d}{dx}(x^2)-\frac{d}{dx}(xy)+\frac{d}{dx}(y^2)
\amp=\amp \displaystyle \frac{d}{dx}(3)
\\[1.2em]
\displaystyle 2x-\bigl(xy'+y\bigr)+2y\,y'
\amp=\amp \displaystyle 0
\\[1.2em]
\displaystyle 2x-y-xy'+2y\,y'
\amp=\amp \displaystyle 0
\\[1.2em]
\displaystyle y'(-x+2y)
\amp=\amp \displaystyle y-2x
\\[1.2em]
\displaystyle y'
\amp=\amp \displaystyle \frac{y-2x}{-x+2y}.
\end{array}
        </me>

        <p>
          At points on the <m>x</m>-axis, <m>y=0</m>, so
        </p>

        <me>
          \displaystyle y'=\frac{-2x}{-x}=2
          \qquad (x\neq 0).
        </me>

        <p>
          In particular, the slope at both <m>(\sqrt{3},0)</m> and <m>(-\sqrt{3},0)</m> is 2, so the tangent lines are parallel.
        </p>
      </solution>
    </example>

    <example xml:id="ex-when-implicit-needed">
      <title>When Do We Need Implicit Differentiation?</title>
      <statement>
        <p>
          Explain how to determine when implicit differentiation is needed to find <m>y'</m>, as opposed to using
          the standard differentiation methods covered earlier. Provide an example where implicit differentiation is required
          and one where it is not.
        </p>
      </statement>

      <solution>
        <p>
          Implicit differentiation is needed when <m>y</m> is not given explicitly as a function of <m>x</m>, or when the equation
          mixes <m>x</m> and <m>y</m> in a way that makes solving for <m>y</m> difficult or undesirable. In these cases, we treat <m>y</m>
          as a function of <m>x</m> and differentiate both sides with respect to <m>x</m>, remembering that derivatives of expressions involving
          <m>y</m> must include a factor of <m>y'</m>.
        </p>

        <p>
          For example, the equation <m>x^2+y^2=25</m> defines a circle. Solving for <m>y</m> gives
          <m>y=\pm\sqrt{25-x^2}</m>, which is possible but splits into two functions. Implicit differentiation gives
          <m>\displaystyle 2x+2y\,y'=0</m>, so <m>\displaystyle y'=-\frac{x}{y}</m>, which works on the whole circle
          (except where <m>y=0</m>).
        </p>

        <p>
          On the other hand, if <m>y</m> is already given explicitly, such as <m>y=(x^2+1)^5</m>, then standard differentiation rules apply directly
          and there is no need for implicit differentiation. In this example, the Chain Rule gives
          <m>\displaystyle y'=5(x^2+1)^4\cdot 2x</m>.
        </p>
      </solution>
    </example>

    <example xml:id="ex-geom-meaning-slope">
      <title>Geometric Meaning of <m>y'=5</m></title>
      <statement>
        <p>
          A student uses implicit differentiation on a curve and finds that <m>y'=5</m> at the point <m>(x,y)=(1,2)</m>.
          Explain the geometric meaning of this result as it relates to the graph of the curve.
        </p>
      </statement>

      <solution>
        <p>
          The derivative <m>y'=5</m> at <m>(1,2)</m> means that the tangent line to the curve at that point has slope 5.
          Geometrically, the curve is increasing at <m>(1,2)</m>, and near that point the graph rises about 5 units vertically
          for every 1 unit horizontally (using the usual interpretation of slope).
        </p>

        <p>
          Equivalently, if we zoom in close enough around <m>(1,2)</m>, the curve looks nearly like the tangent line, and that tangent line has equation


        <me>
          \displaystyle y-2=5(x-1).
        </me>
                </p>
      </solution>
    </example>
  </subsection>

<subsection xml:id="additional-worked-problems-derivImplic">
  <title>Additional Worked-Out Examples</title>

  <p>
    To keep this section at a reasonable length, we include only a few representative examples directly in the text.
    If you find yourself stuck on a homework problem, or if you are studying before a quiz or exam, additional
    fully worked-out examples are available via: 
    <alert>
      <xref ref="subsec-deriv-implicit">
        Additional Examples for Implicit Differentiation
      </xref>
    </alert>
  </p>

</subsection>

</section>
